theories/LogicalRelation/NormalRed.v
@@ -1,126 +1,146 @@
 
+From Coq Require Import CRelationClasses.
 From LogRel.AutoSubst Require Import core unscoped Ast Extra.
-From LogRel Require Import Utils BasicAst Notations LContexts Context NormalForms Weakening GenericTyping LogicalRelation DeclarativeInstance.
+From LogRel Require Import Utils BasicAst Notations LContexts Context NormalForms UntypedReduction Weakening GenericTyping Monad LogicalRelation.
 From LogRel.LogicalRelation Require Import Induction Irrelevance Escape Reflexivity Weakening Neutral Transitivity Reduction.
 
 Set Universe Polymorphism.
+
+Ltac redSubst :=
+  match goal with
+  | [H : [_ |- ?X :⤳*: ?Y]< _ > |- _] => 
+    assert (X = Y)by (eapply redtywf_whnf ; gen_typing); subst; clear H
+  end.
+
 
 Section Normalization.
 Context `{GenericTypingProperties}.
 
 Set Printing Primitive Projection Parameters.
 
+
+Program Definition normRedNe0 {wl Γ A} (h : [Γ ||-ne A]< wl >) (wh : whne A) :
+  [Γ ||-ne A]< wl > :=
+  {| neRedTy.ty := A |}.
+Next Obligation.
+  pose proof (LRne_ zero h); escape; now eapply redtywf_refl.
+Qed.
+Next Obligation. destruct h; now redSubst. Qed.
+
+
+
 Program Definition normRedΠ0 {wl Γ F G l} (h : [Γ ||-Π<l> tProd F G]< wl >)
   : [Γ ||-Π<l> tProd F G]< wl > :=
   {| PiRedTyPack.dom := F ;
-    PiRedTyPack.cod := G |}.
-Obligation 1.
-  intros;
-  assert (wΠ : whnf (tProd F G)) by constructor;
-  pose proof (e := redtywf_whnf (PiRedTyPack.red h) wΠ);
-  symmetry in e; injection e; clear e.
-  destruct h as [?????? domRed codRed codExt] ; 
-    intros; cbn in *; subst; eassumption + now eapply domRed.
-Defined. 
-Obligation 2.
-  intros;
-  assert (wΠ : whnf (tProd F G)) by constructor;
-  pose proof (e := redtywf_whnf (PiRedTyPack.red h) wΠ);
-  symmetry in e; injection e; clear e.
-  destruct h as [?????? domRed codRed codExt] ; 
-    intros; cbn in *; subst; eassumption + now eapply domRed.
-Defined.
-Obligation 3.
+     PiRedTyPack.cod := G |}.
+Solve All Obligations with 
+  intros; pose proof (e := redtywf_whnf (PiRedTyPack.red h) whnf_tProd);
+  symmetry in e; injection e; clear e; 
+  destruct h ; intros; cbn in *; subst; eassumption.
 
-  intros;
-  assert (wΠ : whnf (tProd F G)) by constructor;
-  pose proof (e := redtywf_whnf (PiRedTyPack.red h) wΠ);
-  symmetry in e; injection e; clear e.
-  destruct h as [?????? domRed codRed codExt] ; 
-    intros; cbn in *; subst; eassumption + now eapply domRed.
-Defined.
-Obligation 4.
-  intros;
-  assert (wΠ : whnf (tProd F G)) by constructor;
-  pose proof (e := redtywf_whnf (PiRedTyPack.red h) wΠ);
-  symmetry in e; injection e; clear e.
-  destruct h as [?????? domRed codRed codExt] ; 
-    intros; cbn in *; subst; eassumption + now eapply domRed.
-Defined.
-Obligation 5.
-  destruct h as [??????? domRed codRed codExt] ; 
-    intros; cbn in *; subst. exact domN.
-Defined.
-Obligation 6. 
-  intros;
-  assert (wΠ : whnf (tProd F G)) by constructor;
-  pose proof (e := redtywf_whnf (PiRedTyPack.red h) wΠ);
-  symmetry in e; injection e; clear e.
-  destruct h as [??????? domRed codRed codExt] ; 
-    intros; cbn in *; subst; try eassumption.
-  eapply domRed ; try eassumption.
-Defined.
-Obligation 7.
-  intros;
-  assert (wΠ : whnf (tProd F G)) by constructor;
-  pose proof (e := redtywf_whnf (PiRedTyPack.red h) wΠ);
-  symmetry in e; injection e; clear e.
-  destruct h as [??????? domRed codomN codRed codExt].
-  intros ; cbn in *.
-  unshelve eapply codomN ; try eassumption.
-  subst.
-  now irrelevance.
-Defined.
 
-Obligation 8.
-  intros;
-  assert (wΠ : whnf (tProd F G)) by constructor.
-  pose proof (e := redtywf_whnf (PiRedTyPack.red h) wΠ).
-  symmetry in e; injection e; clear e.
-  destruct h as [??????? domRed codomN codRed codExt] ; 
-    intros; cbn in *.
-  subst.
-  unshelve eapply codRed ;[exact wl' |..] ; tea.
-Defined.
-
-Next Obligation.
-  intros;
-  assert (wΠ : whnf (tProd F G)) by constructor.
-  pose proof (e := redtywf_whnf (PiRedTyPack.red h) wΠ).
-  symmetry in e; injection e; clear e.
-  destruct h as [??????? domRed codomN codRed codExt] ; 
-    intros; cbn in *.
-  subst.
-  irrelevance0 ; try reflexivity.
-  unshelve eapply codExt ; [exact wl' | ..] ; try eassumption ; tea ; irrelevance.
-Qed.
-
+Program Definition normRedΣ0 {wl Γ F G l} (h : [Γ ||-Σ<l> tSig F G]< wl >)
+  : [Γ ||-Σ<l> tSig F G]< wl > :=
+  {| PiRedTyPack.dom := F ;
+     PiRedTyPack.cod := G |}.
+Solve All Obligations with 
+  intros; pose proof (e := redtywf_whnf (PiRedTyPack.red h) whnf_tSig);
+  symmetry in e; injection e; clear e; 
+  destruct h ; intros; cbn in *; subst; eassumption.
   
 Definition normRedΠ {wl Γ F G l} (h : [Γ ||-<l> tProd F G]< wl >)
   : [Γ ||-<l> tProd F G]< wl > :=
   LRPi' (normRedΠ0 (invLRΠ h)).
+
+
+Definition normRedΣ {wl Γ F G l} (h : [Γ ||-<l> tSig F G]< wl >) : [Γ ||-<l> tSig F G]< wl > :=
+  LRSig' (normRedΣ0 (invLRΣ h)).
+
+#[program]
+Definition normEqRedΣ {wl Γ F F' G G' l} (h : [Γ ||-<l> tSig F G]< wl >) 
+  (heq : [Γ ||-<l> _ ≅ tSig F' G' | h]< wl >) : [Γ ||-<l> _ ≅ tSig F' G' | normRedΣ h]< wl > :=
+  {|
+    PiRedTyEq.dom := F';
+    PiRedTyEq.cod := G';
+  |}.
+Solve All Obligations with
+  intros; assert[Γ ||-<l> _ ≅ tSig F' G' | normRedΣ h]< wl > as [?? red] by irrelevance;
+  pose proof (e := redtywf_whnf red whnf_tSig);
+  symmetry in e; injection e; clear e; 
+  destruct h ; intros; cbn in *; subst; eassumption.
 
 #[program]
 Definition normLambda {wl Γ F F' G t l RΠ} 
   (Rlam : [Γ ||-<l> tLambda F' t : tProd F G | normRedΠ RΠ ]< wl >) :
   [Γ ||-<l> tLambda F' t : tProd F G | normRedΠ RΠ ]< wl > :=
   {| PiRedTm.nf := tLambda F' t |}.
+Obligation 3.
+eapply (PiRedTm.appTree Rlam ρ f Hd ha).
+Defined.
 Obligation 5.
-  destruct Rlam as [??????? app eqq]; cbn in *; try exact redN.
+pose proof (e := redtmwf_whnf (PiRedTm.red Rlam) whnf_tLambda).
+destruct Rlam as [????? app eqq].
+eapply (f_equal (ren_term ρ)) in e ; cbn in *.
+rewrite e.
+now eapply app.
 Defined.
-Obligation 6.
-  intros;
-  pose proof (e := redtmwf_whnf (PiRedTm.red Rlam) whnf_tLambda);
-    destruct Rlam as [??????? app eqq]; cbn in *.
-  unshelve eapply appN ; try eassumption ; subst ; try eassumption.
-Defined.
-
 Solve All Obligations with
   intros;
   pose proof (e := redtmwf_whnf (PiRedTm.red Rlam) whnf_tLambda);
-  destruct Rlam as [??????? app eqq]; cbn in *; try exact redN ; subst;
-first [eapply app ; eassumption | now eapply eqq| eassumption].
-  
+  destruct Rlam as [????? app eqq]; cbn in *; subst;
+first [eapply app | now eapply eqq| eassumption].
+
+
+#[program]
+Definition normPair {wl Γ F F' G G' f g l RΣ} 
+  (Rp : [Γ ||-<l> tPair F' G' f g : tSig F G | normRedΣ RΣ ]< wl >) :
+  [Γ ||-<l> tPair F' G' f g : tSig F G | normRedΣ RΣ ]< wl > :=
+  {| SigRedTm.nf := tPair F' G' f g |}.
+Obligation 4.
+eapply (SigRedTm.sndTree Rp) ; eassumption.
+Defined.
+Obligation 5.
+  intros;
+  pose proof (e := redtmwf_whnf (SigRedTm.red Rp) whnf_tPair);
+    destruct Rp as [??? fstRed ?? sndRed]; cbn in * ; now subst.
+Defined.
+Next Obligation.
+  intros;
+    pose proof (e := redtmwf_whnf (SigRedTm.red Rp) whnf_tPair);
+    destruct Rp as [??? fstRed ?? sndRed]; cbn in *; now subst.
+Defined.
+Next Obligation.
+  intros;
+    pose proof (e := redtmwf_whnf (SigRedTm.red Rp) whnf_tPair);
+    destruct Rp as [??? fstRed ?? sndRed]; cbn in *; now subst.
+Defined.
+Next Obligation.
+  intros;
+    pose proof (e := redtmwf_whnf (SigRedTm.red Rp) whnf_tPair);
+    destruct Rp as [??? fstRed ?? sndRed]; cbn in *; subst.
+  now eapply fstRed.
+Defined.
+Next Obligation.
+  intros;
+    destruct Rp as [??? fstRed ?? sndRed]; cbn in *.
+  unfold normPair_obligation_3 in * ; cbn in * ; revert Ho.
+  destruct (redtmwf_whnf red whnf_tPair) ; subst ; cbn in *.
+  intros Ho.
+  irrelevanceRefl ; unshelve eapply sndRed.
+  4,5: eassumption.
+Defined.
+
+Definition invLRcan {wl Γ l A} (lr : [Γ ||-<l> A]< wl >) (w : isType A) : [Γ ||-<l> A]< wl > :=
+  match w as w in isType A return forall (lr : [Γ ||-<l> A]< wl >), invLRTy lr (reflexivity A) w -> [Γ ||-<l> A]< wl > with
+  | UnivType => fun _ x => LRU_ x
+  | ProdType => fun _ x => LRPi' (normRedΠ0 x)
+  | NatType => fun _ x => LRNat_ _ x
+  | BoolType => fun _ x => LRBool_ _ x
+  | EmptyType => fun _ x => LREmpty_  _ x
+  | SigType => fun _ x => LRSig' (normRedΣ0 x)
+  | IdType => fun _ x => LRId' x
+  | NeType wh => fun _ x => LRne_ _ (normRedNe0 x wh)
+  end lr (invLR lr (reflexivity A) w).
 
 End Normalization.
 
@@ -128,20 +148,33 @@ End Normalization.
 
 (* Normalizes a term reducible at a Π type *)
 
-Ltac normRedΠin id X :=
+Ltac normRedΠin X :=
   let g := type of X in
   match g with
   | [ LRAd.pack ?R | _ ||- ?t : _]< _ > =>
-    pose (id := normRedΠ0 (invLRΠ R));
     let X' := fresh X in
     rename X into X' ;
-    assert (X : [_ ||-<_> t : _ | LRPi' id]< _ >) by irrelevance; clear X'
+    assert (X : [_ ||-<_> t : _ | LRPi' (normRedΠ0 (invLRΠ R))]< _ >) by irrelevance; clear X'
+  | [ LRAd.pack ?R | _ ||- _ ≅ ?B]< _ > =>
+    let X' := fresh X in
+    rename X into X' ;
+    assert (X : [_ ||-<_> _ ≅ B | LRPi' (normRedΠ0 (invLRΠ R))]< _ >) by irrelevance; clear X'
+  | [ LRAd.pack ?R | _ ||- ?t ≅ ?u : _]< _ > =>
+    let X' := fresh X in
+    rename X into X' ;
+    assert (X : [_ ||-<_> t ≅ u : _ | LRPi' (normRedΠ0 (invLRΠ R))]< _ >) by irrelevance; clear X'
   end.
 
-Goal forall `{GenericTypingProperties} wl Γ A B l R f (Rf : [Γ ||-<l> f : arr A B | R]< wl >), True.
+Goal forall `{GenericTypingProperties} wl Γ A B l R f X
+  (RABX : [Γ ||-<l> arr A B ≅ X | R]< wl >)
+  (Rf : [Γ ||-<l> f : arr A B | R]< wl >)
+  (Rff : [Γ ||-<l> f ≅ f : arr A B | R]< wl >)
+, True.
 Proof.
   intros.
-  normRedΠin ΠAB Rf.
+  normRedΠin Rf.
+  normRedΠin Rff.
+  normRedΠin RABX.
   constructor.
 Qed.
 
@@ -155,5 +188,24 @@ Ltac normRedΠ id :=
   | [ LRAd.pack ?R | _ ||- ?t : _]< _ > =>
     pose (id := normRedΠ0 (invLRΠ R)); subst G;
     enough [_ ||-<_> t : _ | LRPi' id]< _ > by irrelevance
+  end.
+
+(* Normalizes a term reducible at a Π type *)
+
+Ltac normRedΣin X :=
+  let g := type of X in
+  match g with
+  | [ LRAd.pack ?R | _ ||- ?t : _]< _ > =>
+    let X' := fresh X in
+    rename X into X' ;
+    assert (X : [_ ||-<_> t : _ | LRSig' (normRedΣ0 (invLRΣ R))]< _ >) by irrelevance; clear X'
+  | [ LRAd.pack ?R | _ ||- _ ≅ ?B]< _ > =>
+    let X' := fresh X in
+    rename X into X' ;
+    assert (X : [_ ||-<_> _ ≅ B | LRSig' (normRedΣ0 (invLRΣ R))]< _ >) by irrelevance; clear X'
+  | [ LRAd.pack ?R | _ ||- ?t ≅ ?u : _]< _ > =>
+    let X' := fresh X in
+    rename X into X' ;
+    assert (X : [_ ||-<_> t ≅ u : _ | LRSig' (normRedΣ0 (invLRΣ R))]< _ >) by irrelevance; clear X'
   end.
 
