theories/LogicalRelation/Application.v
@@ -1,7 +1,7 @@
-Require Import PeanoNat.
+
 From LogRel.AutoSubst Require Import core unscoped Ast Extra.
-From LogRel Require Import Utils BasicAst Notations LContexts Context NormalForms Weakening GenericTyping LogicalRelation DeclarativeInstance.
-From LogRel.LogicalRelation Require Import Induction Irrelevance Escape Reflexivity Weakening Neutral Transitivity Reduction NormalRed.
+From LogRel Require Import Utils BasicAst Notations LContexts Context NormalForms Weakening GenericTyping Monad LogicalRelation.
+From LogRel.LogicalRelation Require Import Split Induction Irrelevance Escape Reflexivity Weakening Monotonicity Neutral Transitivity Reduction NormalRed.
 
 Set Universe Polymorphism.
 
@@ -14,552 +14,61 @@ Context `{GenericTypingProperties}.
 
 Set Printing Primitive Projection Parameters.
 
-Record helpTy2 {Γ F G l} (wl : wfLCon) (WN : nat)
-  :=
-  { f : forall (wl' : wfLCon) (tau : wl' ≤ε wl) (ne : AllInLCon WN wl'),
-      wfLCon;
-    ub : forall (wl' : wfLCon) (tau : wl' ≤ε wl) (ne : AllInLCon WN wl'),
-      f wl' tau ne ≤ε wl ;
-    lesser : forall (wl' : wfLCon) (tau : wl' ≤ε wl) (ne : AllInLCon WN wl'),
-      wl' ≤ε f wl' tau ne ;
-    ne : forall (wl' : wfLCon) (tau : wl' ≤ε wl) (ne : AllInLCon WN wl'),
-      AllInLCon WN (f wl' tau ne) ;
-    dom2 : forall (wl' : wfLCon) (tau : wl' ≤ε wl) (ne : AllInLCon WN wl'),
-      term ;
-    cod2 : forall (wl' : wfLCon) (tau : wl' ≤ε wl) (ne : AllInLCon WN wl'),
-      term ;
-    red2 : forall (wl' : wfLCon) (tau : wl' ≤ε wl) (ne : AllInLCon WN wl'),
-      [Γ |-[ ta ] tProd F G :⇒*: tProd (dom2 wl' tau ne) (cod2 wl' tau ne) ]< (f wl' tau ne) > ;
-    domTy2 : forall (wl' : wfLCon) (tau : wl' ≤ε wl) (ne : AllInLCon WN wl'),
-      [Γ |-[ ta ] (dom2 wl' tau ne) ]< (f wl' tau ne) > ;
-    codTy2 : forall (wl' : wfLCon) (tau : wl' ≤ε wl) (ne : AllInLCon WN wl'),
-      [Γ ,, (dom2 wl' tau ne) |-[ ta ] (cod2 wl' tau ne) ]< (f wl' tau ne) > ;
-    eq2 : forall (wl' : wfLCon) (tau : wl' ≤ε wl) (ne : AllInLCon WN wl'),
-      [Γ |-[ ta ] tProd (dom2 wl' tau ne) (cod2 wl' tau ne) ≅
-             tProd (dom2 wl' tau ne) (cod2 wl' tau ne)]< (f wl' tau ne) > ;
-    domN2 : nat ;
-    domRed2 : forall (wl' : wfLCon) (tau : wl' ≤ε wl) (ne : AllInLCon WN wl'),
-    forall (Δ : context) (l' : wfLCon) (ρ : Δ ≤ Γ),
-           l' ≤ε (f wl' tau ne) ->
-           AllInLCon (domN2) l' -> [ |-[ ta ] Δ ]< l' > ->
-           [Δ ||-< l > (dom2 wl' tau ne)⟨ρ⟩ ]< l' > ;
-    codomN2 : forall (wl' : wfLCon) (tau : wl' ≤ε wl) (ne : AllInLCon WN wl'),
-    forall (Δ : context) (a : term) (l' : wfLCon) (ρ : Δ ≤ Γ)
-             (τ : l' ≤ε (f wl' tau ne))
-             (Ninfl : AllInLCon (domN2) l') (h : [ |-[ ta ] Δ ]< l' >),
-      [domRed2 wl' tau ne Δ l' ρ τ Ninfl h | Δ ||- a : (dom2 wl' tau ne)⟨ρ⟩ ]< l' > -> nat ;
-(*    codomN2_Ltrans :
-    forall (wl' : wfLCon) (tau : wl' ≤ε wl) (ne : AllInLCon WN wl'),
-    forall (Δ : context) (a : term) (l' l'' : wfLCon) 
-           (ρ : Δ ≤ Γ)
-           (τ : l' ≤ε (f wl' tau ne))
-           (τ' : l'' ≤ε (f wl' tau ne))
-           (Ninfl : AllInLCon (domN2) l')
-           (Ninfl' : AllInLCon (domN2) l'')
-           (h : [ |-[ ta ] Δ ]< l' >) (h' : [ |-[ ta ] Δ ]< l'' >)
-           (ha : [domRed2 wl' tau ne Δ l' ρ τ Ninfl h | Δ ||- a : (dom2 wl' tau ne)⟨ρ⟩ ]< l' >)
-           (ha' : [domRed2 wl' tau ne Δ l'' ρ τ' Ninfl' h' | Δ ||- a : (dom2 wl' tau ne)⟨ρ⟩ ]< l'' >),
-      l'' ≤ε l' ->
-      codomN2 wl' tau ne Δ a l'' ρ τ' Ninfl' h' ha' <=
-        codomN2 wl' tau ne Δ a l' ρ τ Ninfl h ha ;
-    codomN2_Ltrans' :
-    forall (wl' wl'' : wfLCon) (tau : wl' ≤ε wl) (tau' : wl'' ≤ε wl)
-           (ne : AllInLCon WN wl') (ne' : AllInLCon WN wl''),
-    forall (Δ : context) (a : term) (l': wfLCon) 
-           (ρ : Δ ≤ Γ)
-           (τ : l' ≤ε (f wl' tau ne))
-           (τ' : l' ≤ε (f wl'' tau' ne'))
-           (Ninfl : AllInLCon domN2 l')
-           (h : [ |-[ ta ] Δ ]< l' >)
-           (ha : [domRed2 wl' tau ne Δ l' ρ τ Ninfl h | Δ ||- a : (dom2 wl' tau ne)⟨ρ⟩ ]< l' >)
-           (ha' : [domRed2 wl'' tau' ne' Δ l' ρ τ' Ninfl h | Δ ||- a : (dom2 wl'' tau' ne')⟨ρ⟩ ]< l' >),
-      wl'' ≤ε wl' ->
-      codomN2 wl'' tau' ne' Δ a l' ρ τ' Ninfl h ha' <=
-        codomN2 wl' tau ne Δ a l' ρ τ Ninfl h ha ;*)
-    codRed2 :
-    forall (wl' : wfLCon) (tau : wl' ≤ε wl) (ne : AllInLCon WN wl'),
-    forall (Δ : context) (a : term) (l' : wfLCon) (ρ : Δ ≤ Γ)
-             (τ : l' ≤ε (f wl' tau ne))
-             (Ninfl : AllInLCon (domN2) l')
-             (h : [ |-[ ta ] Δ ]< l' >)
-             (ha : [domRed2 wl' tau ne Δ l' ρ τ Ninfl h | Δ ||- a : (dom2 wl' tau ne)⟨ρ⟩ ]< l' >) 
-             (l'' : wfLCon),
-      l'' ≤ε l' ->
-      AllInLCon (codomN2 wl' tau ne Δ a l' ρ τ Ninfl h ha) l'' ->
-      [Δ ||-< l > (cod2 wl' tau ne)[a .: ρ >> tRel] ]< l'' > ;
-    codExt2 :
-    forall (wl' : wfLCon) (tau : wl' ≤ε wl) (ne : AllInLCon WN wl'),
-    forall (Δ : context) (a b : term) (l' : wfLCon) (ρ : Δ ≤ Γ)
-             (τ : l' ≤ε (f wl' tau ne))
-             (Ninfl : AllInLCon domN2 l')
-             (h : [ |-[ ta ] Δ ]< l' >)
-             (ha : [domRed2 wl' tau ne Δ l' ρ τ Ninfl h | Δ ||- a : (dom2 wl' tau ne)⟨ρ⟩ ]< l' >),
-           [domRed2 wl' tau ne Δ l' ρ τ Ninfl h | Δ ||- b : (dom2 wl' tau ne)⟨ρ⟩ ]< l' > ->
-           [domRed2 wl' tau ne Δ l' ρ τ Ninfl h | Δ ||- a ≅ b : (dom2 wl' tau ne)⟨ρ⟩ ]< l' > ->
-           forall (l'' : wfLCon) (τ' : l'' ≤ε l')
-             (Minfl : AllInLCon (codomN2 wl' tau ne Δ a l' ρ τ Ninfl h ha) l''),
-             [codRed2 wl' tau ne Δ a l' ρ τ Ninfl h ha l'' τ' Minfl |
-               Δ ||- (cod2 wl' tau ne)[a .: ρ >> tRel] ≅
-                 (cod2 wl' tau ne)[b .: ρ >> tRel] ]< l'' > ;
-  }.
-
 
 Section AppTerm.
-  Context {wl Γ t u F G l l'}
+  Context {wl Γ t u F G l l' l''}
     (hΠ : [Γ ||-Π<l> tProd F G]< wl >)
-    {RFN : nat}
-    {RF : forall wl' (τ : wl' ≤ε wl) (Ninfl : AllInLCon RFN wl'),
-        [Γ ||-<l'> F]< wl' > }
-    (Rt : [Γ ||-<l> t : tProd F G | LRPi' (hΠ)]< wl >)
-    (RuN : nat)
-    (Ru : forall wl' (τ : wl' ≤ε wl)
-                 (Ninfl : AllInLCon RFN wl')
-                 (Ninfl' : AllInLCon RuN wl'),
-        [Γ ||-<l'> u : F | RF wl' τ Ninfl ]< wl' >)
-  (*  (RGu : W[Γ ||-<l''> G[u..]]< wl >) *).
-    
-  Definition AppTyN : nat.
-  Proof.
-    refine (max (max (max RFN RuN)
-               (max (PiRedTyPack.domN hΠ) (PiRedTm.redN Rt))) _).
-    unshelve refine (Max_Bar _ _ _).
-    About Max_Bar_Bar_lub.
-    + assumption.
-    + exact (max (max RFN RuN)
-               (max (PiRedTyPack.domN hΠ) (PiRedTm.redN Rt))).
-    + intros.
-      unshelve eapply (PiRedTyPack.codomN hΠ).
-      * assumption.
-      * exact u.
-      * exact wl'.
-      * exact wk_id.
-      * assumption.
-      * (eapply AllInLCon_le ; [ | eassumption] ;
-                  eapply Nat.max_lub_l ;
-                  now eapply Nat.max_lub_r).
-      * eapply wfc_Ltrans ; try eassumption.
-        exact (wfc_wft (PiRedTyPack.domTy hΠ)).
-      * abstract (irrelevance0 ;
-                  [ | unshelve eapply Ru ; try eassumption ;
-                      eapply AllInLCon_le ;
-                      [ eapply Nat.max_lub_l ;
-                        now eapply Nat.max_lub_l | eassumption |
-                        eapply Nat.max_lub_r ;
-                        now eapply Nat.max_lub_l | eassumption]] ;
-         assert (tProd (PiRedTyPack.dom hΠ) (PiRedTyPack.cod hΠ) =
-                   tProd F G) as ePi ;
-         [pose proof (eq := (PiRedTyPack.red hΠ)) ;
-          eapply whredty_det ; now gen_typing |
-           inversion ePi ; now bsimpl]).
-  Defined.
-About AppTyN_subproof.
-    
+    {RF : [Γ ||-<l'> F]< wl >}
+    (Rt : [Γ ||-<l> t : tProd F G | LRPi' (normRedΠ0 hΠ)]< wl >)
+    (Ru : [Γ ||-<l'> u : F | RF]< wl >)
+    (RGu : W[Γ ||-<l''> G[u..]]< wl >).
 
-  Definition AppTy : W[Γ ||-<l> G[u..]]< wl >.
+  Lemma app_id : W[Γ ||-<l''> tApp (PiRedTm.nf Rt) u : G[u..] | RGu]< wl >.
   Proof.
-    exists AppTyN.
-    pose proof (r:= PiRedTyPack.red hΠ). 
-    assert (tProd (PiRedTyPack.dom hΠ) (PiRedTyPack.cod hΠ) = tProd F G) as ePi
-        by (eapply whredty_det ; gen_typing) ; clear r.
-    inversion ePi ; subst ; clear ePi.
-    pose proof (wfΓ := wfc_wft (PiRedTyPack.domTy hΠ)).
-    intros.
-    replace ((PiRedTyPack.cod hΠ)[u..]) with ((PiRedTyPack.cod hΠ)[u .: _wk_id Γ >> tRel]) by now bsimpl.
-    unshelve eapply ((PiRedTyPack.codRed hΠ) wk_id).
-    - unshelve eapply (Bar_lub wl wl' _ τ).
-      exact (max (max RFN RuN)
-               (max (PiRedTyPack.domN hΠ) (PiRedTm.redN Rt))).
-      (eapply AllInLCon_le ; try eassumption ;
-                unfold AppTyN ;
-                now eapply Nat.le_max_l).
-    - now eapply Bar_lub_ub.
-    - (eapply AllInLCon_le ; [ | now eapply Bar_lub_AllInLCon] ;
-                  eapply Nat.max_lub_l ;
-                  now eapply Nat.max_lub_r).
-    - (eapply (wfc_Ltrans)).
-      2: exact (wfc_wft (PiRedTyPack.domTy hΠ)).
-      now eapply Bar_lub_ub.
-    - now eapply (AppTyN_subproof).
-    - now eapply Bar_lub_smaller.
-    - cbn.
-      eapply AllInLCon_le.
-      2: eassumption.
-      unfold AppTyN.
-      etransitivity.
-      2: now eapply Nat.max_lub_r.
-      etransitivity.
-      2: { unshelve eapply (Max_Bar_Bar_lub).
-           2: eassumption.
-           + (eapply AllInLCon_le ; try eassumption ;
-                unfold AppTyN ;
-                now eapply Nat.le_max_l).
-           + now eapply Bar_lub_ub. 
-           + now eapply Bar_lub_AllInLCon.
-      }
-      reflexivity.
-      Defined. 
-      
-  Definition app_idN : nat.
-  Proof.
-    refine (max (max (max RFN RuN) (max (PiRedTyPack.domN hΠ) (PiRedTm.redN Rt))) _).
-    unshelve eapply Max_Bar.
-    - exact wl.
-    - exact (max (max RFN RuN) (max (PiRedTyPack.domN hΠ) (PiRedTm.redN Rt))).
-    - intros.
-      unshelve eapply (PiRedTm.appN Rt).
-      + assumption.
-      + exact u.
-      + exact wl'.
-      + now eapply wk_id.
-      + assumption.
-      + (eapply AllInLCon_le ; [ | eassumption] ;
-                  eapply Nat.max_lub_l ;
-         now eapply Nat.max_lub_r).
-      + eapply wfc_Ltrans ; try eassumption.
-        exact (wfc_wft (PiRedTyPack.domTy hΠ)).
-      + eapply AllInLCon_le ; [ | eassumption].
-        eapply Nat.max_lub_r ; now eapply Nat.max_lub_r.
-      + eapply AppTyN_subproof.
-Defined.
-  
-  Lemma app_id_aux :
-    W[Γ ||-<l> tApp (PiRedTm.nf Rt) u : G[u..] | AppTy]< wl >.
-  Proof.
-    exists app_idN.
-    intros.
+    assert (wfΓ := wfc_wft (escape RF)).
     replace (PiRedTm.nf _) with (PiRedTm.nf Rt)⟨@wk_id Γ⟩ by now bsimpl.
-    irrelevance0.  2: unshelve eapply (PiRedTm.app Rt).
-    cbn.
-    abstract (assert (tProd (PiRedTyPack.dom hΠ) (PiRedTyPack.cod hΠ) = tProd F G) as ePi ;
-              [ pose proof (red := (PiRedTyPack.red hΠ)) ;
-                eapply whredty_det ; now gen_typing |
-                inversion ePi ; subst ; 
-                now bsimpl]).
-    - unshelve eapply (Bar_lub wl wl' _ τ).
-      + exact (max (max RFN RuN) (max (PiRedTyPack.domN hΠ) (PiRedTm.redN Rt))).
-      + (eapply AllInLCon_le ; try eassumption ;
-                unfold AppTyN ;
-                now eapply Nat.le_max_l).
-    - now eapply Bar_lub_ub.
-    - (eapply AllInLCon_le ; [ | now eapply Bar_lub_AllInLCon] ;
-                  eapply Nat.max_lub_l ;
-       now eapply Nat.max_lub_r).
-    - (eapply (wfc_Ltrans)).
-      2: exact (wfc_wft (PiRedTyPack.domTy hΠ)).
-      now eapply Bar_lub_ub.
-    - eapply AppTyN_subproof.
-    - now eapply Bar_lub_smaller.
-    - cbn.
-      unfold NormalRed.normRedΠ0_obligation_7.
-      cbn.
-      eapply AllInLCon_le ; [ | exact Ninfl].
-      unfold AppTy ; cbn ; unfold AppTyN ; cbn.
-      etransitivity.
-      2:{eapply Nat.max_lub_r.
-         cbn ; unfold AppTyN.
-         reflexivity. }
-      etransitivity.
-      2:{ unshelve eapply (Max_Bar_Bar_lub).
+    unshelve econstructor.
+    - eapply DTree_fusion.
+      + unshelve eapply (PiRedTm.appTree Rt wk_id (wfLCon_le_id _)).
+        2: eassumption.
+        * exact u.
+        * cbn in *.
+          irrelevance0.
           2: eassumption.
-          + (eapply AllInLCon_le ; try eassumption ;
-                unfold AppTyN ;
-                now eapply Nat.le_max_l).
-          + now eapply Bar_lub_ub.
-          + now eapply Bar_lub_AllInLCon.
-          + clear Ninfl Ninfl' τ wl'.
-             (intros ;
-              rewrite (AllInLCon_Irrel _ _ ne0 ne') ;
-              rewrite (wfLCon_le_Irrel _ _ τ τ');
-              reflexivity). }
-      reflexivity.
-    - eapply AllInLCon_le.
-      2: eapply Bar_lub_AllInLCon.
-      eapply Nat.max_lub_r ; now eapply Nat.max_lub_r. 
-    - cbn.
-      eapply AllInLCon_le ; [ | eassumption].
-      etransitivity.
-      2:{unfold app_idN.
-         eapply Nat.max_lub_r.
-         reflexivity. }
-      etransitivity.
-      2:{ unshelve eapply Max_Bar_Bar_lub.
-          + exact wl'.
-          + assumption.
-          + (eapply AllInLCon_le ; try eassumption ;
-                unfold AppTyN ;
-                now eapply Nat.le_max_l). 
-          + now eapply Bar_lub_ub.
-          + cbn. now eapply Bar_lub_AllInLCon.
-          + clear Ninfl Ninfl' τ wl'.
-            intros ;
-              rewrite (AllInLCon_Irrel _ _ ne0 ne') ;
-              rewrite (wfLCon_le_Irrel _ _ τ τ');
-              reflexivity.
-      }
-      cbn.
-      reflexivity.
-Qed.        
-
-  Lemma app_id {l''} (RGu : W[Γ ||-<l''> G[u..]]< wl >):
-    W[Γ ||-<l''> tApp (PiRedTm.nf Rt) u : G[u..] | RGu]< wl >.
-  Proof.
-    eapply WLRTmRedIrrelevantCum.
-    exact app_id_aux.
+          now bsimpl.
+      + eapply (PolyRedPack.posTree (normRedΠ0 hΠ) wk_id (wfLCon_le_id _) wfΓ).
+        irrelevance0.
+        2: eassumption.
+        cbn ; now bsimpl.
+    - intros.
+      irrelevance0.
+      2: unshelve eapply (PiRedTm.app Rt wk_id (wfLCon_le_id _) wfΓ).
+      cbn; now bsimpl.
+      2: now eapply over_tree_fusion_r.
+      now eapply over_tree_fusion_l.
   Qed.
-
-  Lemma WappTerm0 {l''} (RGu : W[Γ ||-<l''> G[u..]]< wl >):
+  
+  Lemma appTerm0 :
       W[Γ ||-<l''> tApp t u : G[u..] | RGu]< wl >
       × W[Γ ||-<l''> tApp t u ≅ tApp (PiRedTm.nf Rt) u : G[u..] | RGu]< wl >.
   Proof.
-    Print redwfSubstTerm.
-    split.
-    - destruct (app_id RGu).
-      exists (max (max RuN WNTm) RFN).
-      intros.
-      eapply redwfSubstTerm.
-      + eapply WRedTm ; try eassumption.
-        eapply AllInLCon_le ; [ | exact Ninfl'].
-        eapply Nat.max_lub_r ; now eapply Nat.max_lub_l.
-      + escape.
-        unshelve eapply redtmwf_app ; [ exact F |..].
-        destruct Rt ; cbn in *.
-        destruct hΠ ; cbn in *.
-        split.
-        * eapply ty_Ltrans ; try eassumption.
-          destruct red.
-          eapply ty_exp.
-          -- eassumption.
-          -- now destruct red0.
-        * eapply redtm_Ltrans ; try eassumption.
-          eapply redtm_conv.
-          -- now destruct red.
-          -- unshelve eapply convty_exp.
-             5 : exact eq0.
-             ++ eapply redty_refl.
-                gen_typing.
-             ++ now destruct red0. 
-        * eapply escapeTerm.
-          unshelve eapply Ru ; try eassumption.
-          eapply AllInLCon_le ; [ | exact Ninfl'].
-          now eapply Nat.max_lub_r.
-          eapply AllInLCon_le ; [ | exact Ninfl'].
-          eapply Nat.max_lub_l ; now eapply Nat.max_lub_l.
-    - destruct (app_id RGu).
-      exists (max (max RuN WNTm) RFN).
-      intros.
-      eapply redwfSubstTerm.
-      + eapply WRedTm ; try eassumption.
-        eapply AllInLCon_le ; [ | exact Ninfl'].
-        eapply Nat.max_lub_r ; now eapply Nat.max_lub_l.
-      + escape.
-        eapply redtmwf_app.
-        destruct Rt ; cbn in *.
-        destruct hΠ ; cbn in *.
-        split.
-        * eapply ty_Ltrans ; try eassumption.
-          destruct red.
-          eapply ty_exp.
-          -- eassumption.
-          -- now destruct red0.
-        * eapply redtm_Ltrans ; try eassumption.
-          eapply redtm_conv.
-          -- now destruct red.
-          -- unshelve eapply convty_exp.
-             5 : exact eq0.
-             ++ eapply redty_refl.
-                gen_typing.
-             ++ now destruct red0. 
-        * eapply escapeTerm.
-          unshelve eapply Ru ; try eassumption.
-          eapply AllInLCon_le ; [ | exact Ninfl'].
-          now eapply Nat.max_lub_r.
-          eapply AllInLCon_le ; [ | exact Ninfl'].
-          eapply Nat.max_lub_l ; now eapply Nat.max_lub_l.
+    eapply WredSubstTerm.
+    1: unshelve eapply app_id; tea.
+    escape.
+    eapply redtmwf_app.
+    1: apply Rt.
+    easy.
   Qed.
   
-
 End AppTerm.
-
-
-Definition help {wl Γ F G l} (WN : nat)
-  (WRed : forall wl' : wfLCon, wl' ≤ε wl ->
-                               AllInLCon WN wl' ->
-                               [Γ ||-Π< l > tProd F G ]< wl' >) :
-  helpTy2 (Γ := Γ) (F := F) (G := G) (l := l) wl WN.
-Proof.
-  unshelve econstructor.
-  - intros wl' τ Ninfl.
-    exact (Bar_lub wl wl' WN τ Ninfl).
-  - intros.
-    refine (PiRedTyPack.dom _).
-    unshelve eapply WRed.
-    unshelve eapply Bar_lub_ub ; try eassumption.
-    unshelve eapply Bar_lub_AllInLCon.
-  - intros.
-    refine (PiRedTyPack.cod _).
-    unshelve eapply WRed.
-    unshelve eapply Bar_lub_ub ; try eassumption.
-    unshelve eapply Bar_lub_AllInLCon.
-  - intros.
-    unshelve eapply Max_Bar.
-    + exact wl.
-    + exact WN.
-    + intros * tau Ninfl.
-      refine (PiRedTyPack.domN _).
-      unshelve eapply WRed ; try eassumption.
-  - cbn.
-    intros * τ Ninfl h.
-    refine (PiRedTyPack.domRed _ _ _ _ _) ; try eassumption.
-    eapply AllInLCon_le ; [ | exact Ninfl].
-    unshelve eapply
-      (Max_Bar_Bar_lub _ _ (fun wl'0 tau0 Ninfl0 =>
-                              PiRedTyPack.domN (WRed wl'0 tau0 Ninfl0))).
-    (intros ;
-     rewrite (AllInLCon_Irrel _ _ ne1 ne') ;
-     now rewrite (wfLCon_le_Irrel _ _ τ0 τ')).
-  - cbn.
-    intros * ha.
-    refine (PiRedTyPack.codomN _ _ _ _ _ _) ; try eassumption.
-  - cbn.
-    intros * τ' Minfl.
-    refine (PiRedTyPack.codRed _ _ _ _ _ _ _ _) ; try eassumption.
-  - cbn.
-    intros.
-    now eapply Bar_lub_ub.
-  - cbn ; intros.
-    now eapply Bar_lub_smaller.
-  - cbn ; intros.
-    now eapply Bar_lub_AllInLCon.
-  - cbn.
-    intros.
-    refine (PiRedTyPack.red _) ; try eassumption.
-  - cbn.
-    intros.
-    refine (PiRedTyPack.domTy _) ; try eassumption.
-  - cbn.
-    intros.
-    refine (PiRedTyPack.codTy _) ; try eassumption.
-  - cbn.
-    intros.
-    refine (PiRedTyPack.eq _) ; try eassumption.
-  - cbn ; intros * hb hab *.
-    eapply (PiRedTyPack.codExt _) ; try eassumption.
-Qed.
-
-Lemma test {wl Γ F G l}
-  (RΠ : W[Γ ||-<l> tProd F G]< wl >)
-  : [Γ ||-Π< l > tProd F G ]< wl >.
-Proof.
-  destruct RΠ.
-  destruct (help _ (fun wl' tau Ninfl => invLRΠ (WRed wl' tau Ninfl))).
-  assert (forall (wl' : wfLCon) (tau : wl' ≤ε wl) (ne : AllInLCon WN wl'),
-             tProd F G = tProd (dom3 wl' tau ne) (cod3 wl' tau ne)) as ePi.
-  intros.
-  1:{ now eapply whredty_det ; gen_typing . }
-  unshelve econstructor.
-  - exact F.
-  - exact G.
-  - exact (max WN domN3).
-  - intros * ? ? h.
-    eapply LRCumulative'.
-    2: {unshelve eapply domRed3 ; try eassumption.
-        + eapply AllInLCon_le ; [ | exact Ninfl].
-          now eapply Nat.le_max_l.
-        + now eapply lesser0.
-        + eapply AllInLCon_le ; [ | exact Ninfl].
-          now eapply Nat.le_max_r. }
-    + abstract
-        (specialize ePi with wl' τ (AllInLCon_le WN (Init.Nat.max WN domN3) (Nat.le_max_l WN domN3) wl' Ninfl) ;
-         now inversion ePi).
-  - cbn.
-    intros.
-    unshelve eapply codomN3 ; try eassumption.
-     + eapply AllInLCon_le ; [ | exact Ninfl].
-          now eapply Nat.le_max_l.
-     + now eapply lesser0.
-     + eapply AllInLCon_le ; [ | exact Ninfl].
-       now eapply Nat.le_max_r.
-     + irrelevance0.
-       2: exact ha.
-       exact (eq_sym (test_subproof wl Γ F G WN dom3 cod3 domN3 ePi Δ wl' ρ τ Ninfl)).
-  - cbn.
-    intros.
-    eapply LRCumulative'.
-    2:{ unshelve eapply codRed3.
-        4 : exact τ.
-        9 : exact τ'.
-        all : try eassumption. }
-    abstract
-      (pose proof (ePi' := ePi wl' τ (AllInLCon_le WN (Init.Nat.max WN domN3) (Nat.le_max_l WN domN3) wl' Ninfl)) ; now inversion ePi').
-  - econstructor.
-    2: eapply redty_refl .
-    all: unshelve eapply wft_ϝ_Bar ; try exact WN.
-    all: intros * f allinl.
-    all: unshelve eapply wft_Ltrans ; try exact (f0 wl' f allinl).
-    all: try now eapply lesser0.
-    all: destruct (red3 wl' f allinl).
-    all: now eapply redty_ty_src.
-  - unshelve eapply wft_ϝ_Bar ; try exact WN.
-    intros * f allinl.
-    unshelve eapply wft_Ltrans ; try exact (f0 wl' f allinl).
-    1: now eapply lesser0.
-    replace F with (dom3 wl' f allinl).
-    1: now eapply domTy3.
-    abstract
-        (specialize ePi with wl' f allinl ;
-         now inversion ePi).
-  - unshelve eapply wft_ϝ_Bar ; try exact WN.
-    intros * f allinl.
-    unshelve eapply wft_Ltrans ; try exact (f0 wl' f allinl).
-    1: now eapply lesser0.
-    replace F with (dom3 wl' f allinl).
-    replace G with (cod3 wl' f allinl).
-    1: now eapply codTy3.
-    all: abstract
-        (specialize ePi with wl' f allinl ;
-         now inversion ePi).
-  - unshelve eapply convty_ϝ_Bar ; try exact WN.
-    intros * f allinl.
-    unshelve eapply convty_Ltrans ; try exact (f0 wl' f allinl).
-    1: now eapply lesser0.
-    replace (tProd F G) with (tProd (dom3 wl' f allinl) (cod3 wl' f allinl)).
-    1: now eapply eq3.
-    now eapply (eq_sym (ePi _ _ _)).
-  - cbn.
-    intros * hb hab *.
-    pose proof (ePi' := ePi wl' τ (AllInLCon_le WN (Init.Nat.max WN domN3) (Nat.le_max_l WN domN3) wl' Ninfl)) ; inversion ePi' ; subst.
-    irrelevance0.
-    2:{ unshelve eapply codExt3.
-        9 : irrelevance0 ; [ | exact hb] ; reflexivity.
-        8: irrelevance0 ; [ | exact hab] ; reflexivity.
-        all: try eassumption.
-    }
-    reflexivity.
-Qed.
-      
-  
-
-Lemma appTerm {wl Γ t u F G l}
-  (RΠ : W[Γ ||-<l> tProd F G]< wl >)
-  {RF : W[Γ ||-<l> F]< wl >}
-  (Rt : W[Γ ||-<l> t : tProd F G | RΠ]< wl >)
-  (Ru : W[Γ ||-<l> u : F | RF]< wl >)
-  (RGu : W[Γ ||-<l> G[u..]]< wl >) : 
-  W[Γ ||-<l> tApp t u : G[u..]| RGu]< wl >.
-Proof.
-  unshelve eapply WappTerm0.
-  4: now eapply test.
-  8: irrelevance.
-
-
 
 Lemma appTerm {wl Γ t u F G l}
   (RΠ : [Γ ||-<l> tProd F G]< wl >)
   {RF : [Γ ||-<l> F]< wl >}
   (Rt : [Γ ||-<l> t : tProd F G | RΠ]< wl >)
   (Ru : [Γ ||-<l> u : F | RF]< wl >)
-  (RGu : [Γ ||-<l> G[u..]]< wl >) : 
-  [Γ ||-<l> tApp t u : G[u..]| RGu]< wl >.
+  (RGu : W[Γ ||-<l> G[u..]]< wl >) : 
+  W[Γ ||-<l> tApp t u : G[u..]| RGu]< wl >.
 Proof.  
   unshelve eapply appTerm0.
   7:irrelevance.
@@ -568,7 +77,71 @@ Proof.
   irrelevance.
 Qed.
 
+Lemma WappTerm {wl Γ t u F G l}
+  (hΠ : W[Γ ||-<l> tProd F G]< wl >)
+  {RF : W[Γ ||-<l> F]< wl >}
+  (Rt : W[Γ ||-<l> t : tProd F G | hΠ]< wl >)
+  (Ru : W[Γ ||-<l> u : F | RF]< wl >)
+  (RGu : W[Γ ||-<l> G[u..]]< wl >):
+  W[Γ ||-<l> tApp t u : G[u..] | RGu]< wl >.
+Proof.
+  revert RGu.
+  pattern wl.
+  unshelve eapply split_to_over_tree.
+  2:{ intros wl' n ne Ht Hf RGu.
+      unshelve eapply (TmSplit' (ne := ne)).
+      1,2: eapply WLtrans ; [ | eassumption].
+      1,2: eapply LCon_le_step ; now eapply wfLCon_le_id.
+      + unshelve eapply Ht.
+      + unshelve eapply Hf.
+  } 
+  - eapply DTree_fusion ; eapply DTree_fusion.
+    + exact (WT _ hΠ).
+    + exact (WT _ RF).
+    + exact (WTTm _ Rt).
+    + exact (WTTm _ Ru).
+  - intros wl' Hover.
+    unshelve eapply appTerm.
+    2: eapply (WRed _ hΠ).
+    + now eapply over_tree_fusion_l, over_tree_fusion_l.
+    + eapply (WRed _ RF).
+      now eapply over_tree_fusion_r, over_tree_fusion_l.
+    + eapply (WRedTm _ Rt).
+      now eapply over_tree_fusion_l, over_tree_fusion_r.
+    + eapply (WRedTm _ Ru).
+      now eapply over_tree_fusion_r, over_tree_fusion_r.
+Qed.
 
+Lemma appTerm' {wl Γ t u F G l X}
+  (hΠ : [Γ ||-<l> tProd F G]< wl >)
+  {RF : [Γ ||-<l> F]< wl >}
+  (Rt : [Γ ||-<l> t : tProd F G | hΠ]< wl >)
+  (Ru : [Γ ||-<l> u : F | RF]< wl >)
+  (eq : X = G[u..])
+  (RX : W[Γ ||-<l> X]< wl >) :
+  W[Γ ||-<l> tApp t u : X | RX]< wl >.
+Proof.
+  eapply WLRTmRedIrrelevant' ; [symmetry; tea|].
+  unshelve eapply appTerm; cycle 1; tea.
+  Unshelve. now rewrite <- eq.
+Qed.
+
+
+Lemma WappTerm' {wl Γ t u F G l X}
+  (hΠ : W[Γ ||-<l> tProd F G]< wl >)
+  {RF : W[Γ ||-<l> F]< wl >}
+  (Rt : W[Γ ||-<l> t : tProd F G | hΠ]< wl >)
+  (Ru : W[Γ ||-<l> u : F | RF]< wl >)
+  (eq : X = G[u..])
+  (RX : W[Γ ||-<l> X]< wl >) :
+  W[Γ ||-<l> tApp t u : X | RX]< wl >.
+Proof.
+  eapply WLRTmRedIrrelevant' ; [symmetry; tea|].
+  unshelve eapply WappTerm; cycle 1; tea.
+  Unshelve. now rewrite <- eq.
+Qed.
+
+  
 Lemma appcongTerm {wl Γ t t' u u' F G l l'}
   (RΠ : [Γ ||-<l> tProd F G]< wl >) 
   {RF : [Γ ||-<l'> F]< wl >}
@@ -576,47 +149,152 @@ Lemma appcongTerm {wl Γ t t' u u' F G l l'}
   (Ru : [Γ ||-<l'> u : F | RF]< wl >)
   (Ru' : [Γ ||-<l'> u' : F | RF]< wl >)
   (Ruu' : [Γ ||-<l'> u ≅ u' : F | RF ]< wl >)
-  (RGu : [Γ ||-<l'> G[u..]]< wl >)
+  (RGu : W[Γ ||-<l'> G[u..]]< wl >)
    :
-    [Γ ||-<l'> tApp t u ≅ tApp t' u' : G[u..] | RGu]< wl >.
+   W[Γ ||-<l'> tApp t u ≅ tApp t' u' : G[u..] | RGu]< wl >.
 Proof.
   set (hΠ := invLRΠ RΠ); pose (RΠ' := LRPi' (normRedΠ0 hΠ)).
-  assert [Γ ||-<l> t ≅ t' : tProd F G | RΠ']< wl > as [Rt Rt' ? eqApp] by irrelevance.
+  assert [Γ ||-<l> t ≅ t' : tProd F G | RΠ']< wl > as [Rt Rt' ?? eqApp] by irrelevance.
   set (h := invLRΠ _) in hΠ.
   epose proof (e := redtywf_whnf (PiRedTyPack.red h) whnf_tProd); 
   symmetry in e; injection e; clear e; 
-  destruct h as [?????? domRed codRed codExt] ; clear RΠ Rtt'; 
+  destruct h as [?????? [?? domRed ? codRed codExt]] ; clear RΠ Rtt'; 
   intros; cbn in *; subst. 
   assert (wfΓ : [|-Γ]< wl >) by gen_typing.
-  assert [Γ ||-<l> u' : F⟨@wk_id Γ⟩ | domRed _ (@wk_id Γ) wfΓ]< wl > by irrelevance.
-  assert [Γ ||-<l> u : F⟨@wk_id Γ⟩ | domRed _ (@wk_id Γ) wfΓ]< wl > by irrelevance.
-  assert (RGu' : [Γ ||-<l> G[u'..]]< wl >).
+  assert [Γ ||-<l> u' : F⟨@wk_id Γ⟩ | domRed _ _ (@wk_id Γ) (idε _) wfΓ]< wl > by irrelevance.
+  assert [Γ ||-<l> u : F⟨@wk_id Γ⟩ | domRed _ _ (@wk_id Γ) (idε _) wfΓ]< wl > by irrelevance.
+  assert (RGu' : W[Γ ||-<l> G[u'..]]< wl >).
   1:{
     replace G[u'..] with G[u' .: @wk_id Γ >> tRel] by now bsimpl.
-    now eapply (codRed _ u' (@wk_id Γ)).
+    exists (posTree _ _ u' (@wk_id Γ) (idε _) wfΓ X).
+    intros wl' f.
+    eapply (codRed _ u' _ (@wk_id Γ) (idε _)).
+    eassumption.
   }
-  assert (RGuu' : [Γ ||-<l>  G [u'..] ≅ G[u..]  | RGu']< wl >).
+  assert (RGuu' : W[Γ ||-<l>  G [u'..] ≅ G[u..]  | RGu']< wl >).
   1:{
     replace G[u..] with G[u .: @wk_id Γ >> tRel] by now bsimpl.
-    irrelevance0.
-    2: unshelve eapply codExt.
-    6: eapply LRTmEqSym; irrelevance.
-    2-4: tea.
-    now bsimpl.
+    unshelve eapply WLRTyEqIrrelevant'.
+    5: exists (posTree _ _ u' (@wk_id Γ) (idε _) wfΓ X) ; intros wl' f Hover.
+    5: irrelevance0 ; [ reflexivity | ].
+    5: unshelve eapply codExt.
+    11: eapply LRTmEqSym; irrelevance.
+    4-8: tea.
+    3: now bsimpl.
+    2: now replace G[u' .: @wk_id Γ >> tRel] with G[u'..] by now bsimpl.
   }
-  eapply transEqTerm; eapply transEqTerm.
-  - eapply (snd (appTerm0 hΠ Rt Ru RGu)).
-  - unshelve epose  proof (eqApp _ u (@wk_id Γ) wfΓ _).  1: irrelevance. 
+  pose (fez:= (snd (appTerm0 hΠ Rt Ru RGu))).
+  pose (zef := (snd (appTerm0 hΠ Rt' Ru' RGu'))).
+  unshelve epose  proof (eqApp _ u _ (@wk_id Γ) (idε _) wfΓ _).  1: irrelevance.
+  cbn in *.
+  eapply WtransEqTerm; eapply WtransEqTerm.
+  - unshelve eapply (snd (appTerm0 hΠ Rt Ru RGu)).
+  - unshelve epose  proof (eqApp _ u _ (@wk_id Γ) (idε _) wfΓ _).  1: irrelevance.
     replace (PiRedTm.nf Rt) with (PiRedTm.nf Rt)⟨@wk_id Γ⟩ by now bsimpl.
-    irrelevance.
-  - unshelve epose proof (PiRedTm.eq Rt' (a:= u) (b:=u') (@wk_id Γ) wfΓ _ _ _).
-    all: irrelevance.
+    unshelve econstructor.
+    2:intros wl' Hover Hover' ; irrelevance0 ; [ | unshelve eapply X2].
+    2: now bsimpl.
+    3: eapply over_tree_fusion_l ; exact Hover'. 
+    eapply over_tree_fusion_r ; exact Hover'.
+  - unshelve epose proof (Hyp := PiRedTm.eq Rt' (a:= u) (b:=u') (@wk_id Γ) (idε wl) wfΓ _ _).
+    3: unshelve econstructor ; [ | intros wl' Hover Hover' ; irrelevance0].
+    5: unshelve eapply Hyp.
+    4: now bsimpl.
+    1,2,5: irrelevance.
+    2: eapply over_tree_fusion_l ; exact Hover'. 
+    eapply over_tree_fusion_r ; exact Hover'.
   - replace (_)⟨_⟩ with (PiRedTm.nf Rt') by now bsimpl.
-    eapply LRTmEqRedConv; tea.
-    eapply LRTmEqSym.
+    eapply WLRTmEqRedConv; tea.
+    eapply WLRTmEqSym.
     eapply (snd (appTerm0 hΠ Rt' Ru' RGu')).
 Qed.
 
+
+Lemma WappcongTerm {wl Γ t t' u u' F G l l'}
+  (RΠ : W[Γ ||-<l> tProd F G]< wl >) 
+  {RF : W[Γ ||-<l'> F]< wl >}
+  (Rtt' : W[Γ ||-<l> t ≅ t' : tProd F G | RΠ]< wl >)
+  (Ru : W[Γ ||-<l'> u : F | RF]< wl >)
+  (Ru' : W[Γ ||-<l'> u' : F | RF]< wl >)
+  (Ruu' : W[Γ ||-<l'> u ≅ u' : F | RF ]< wl >)
+  (RGu : W[Γ ||-<l'> G[u..]]< wl >)
+   :
+   W[Γ ||-<l'> tApp t u ≅ tApp t' u' : G[u..] | RGu]< wl >.
+Proof.
+  revert RGu.
+  pattern wl.
+  unshelve eapply split_to_over_tree.
+  - do 2 (eapply DTree_fusion) ; [eapply DTree_fusion | eapply DTree_fusion | ..].
+    + exact (WT _ RΠ).
+    + exact (WT _ RF).
+    + exact (WTTmEq _ Rtt').
+    + exact (WTTm _ Ru).
+    + exact (WTTm _ Ru').
+    + exact (WTTmEq _ Ruu').
+  - intros wl' n ne Ht Hf RGu.
+    eapply WLRTmEqIrrelevant' ; [reflexivity | unshelve eapply TmEqSplit].
+    2: exact ne.
+    1,2: eapply WLtrans ; [ | eassumption].
+    1,2: eapply LCon_le_step ; now eapply wfLCon_le_id.
+    + now apply Ht.
+    + now apply Hf.
+  - intros wl' Hover RGu.
+    unshelve eapply appcongTerm.
+    3: unshelve eapply (WRed _ RΠ).
+    + now do 3 (eapply over_tree_fusion_l).
+    + eapply (WRed _ RF).
+      now eapply over_tree_fusion_r ; do 2 (eapply over_tree_fusion_l).
+    + eapply (WRedTmEq _ Rtt').
+      now eapply over_tree_fusion_l, over_tree_fusion_r, over_tree_fusion_l.
+    + eapply (WRedTm _ Ru).
+      now eapply over_tree_fusion_r, over_tree_fusion_r, over_tree_fusion_l.
+    + eapply (WRedTm _ Ru').
+      now eapply over_tree_fusion_l, over_tree_fusion_r.
+    + eapply (WRedTmEq _ Ruu').
+      now eapply over_tree_fusion_r, over_tree_fusion_r.
+Qed.
+  
+
+Lemma appcongTerm' {wl Γ t t' u u' F F' G l l' X}
+  (RΠ : [Γ ||-<l> tProd F G]< wl >) 
+  {RF : [Γ ||-<l'> F]< wl >}
+  {RF' : [Γ ||-<l'> F']< wl >}
+  (RFF' : [Γ ||-<l'> F ≅ F' | RF]< wl >)
+  (Rtt' : [Γ ||-<l> t ≅ t' : tProd F G | RΠ]< wl >)
+  (Ru : [Γ ||-<l'> u : F | RF]< wl >)
+  (Ru' : [Γ ||-<l'> u' : F' | RF']< wl >)
+  (Ruu' : [Γ ||-<l'> u ≅ u' : F | RF ]< wl >)
+  (RGu : W[Γ ||-<l'> X]< wl >)
+   : X = G[u..] ->
+    W[Γ ||-<l'> tApp t u ≅ tApp t' u' : X | RGu]< wl >.
+Proof.
+  intros eq.
+  eapply WLRTmEqIrrelevant' ; [symmetry; apply eq|].
+  eapply appcongTerm; tea.
+  eapply LRTmRedConv; tea.
+  now eapply LRTyEqSym.
+  Unshelve. now rewrite <- eq.
+Qed.
+
+Lemma WappcongTerm' {wl Γ t t' u u' F F' G l l' X}
+  (RΠ : W[Γ ||-<l> tProd F G]< wl >) 
+  {RF : W[Γ ||-<l'> F]< wl >}
+  {RF' : W[Γ ||-<l'> F']< wl >}
+  (RFF' : W[Γ ||-<l'> F ≅ F' | RF]< wl >)
+  (Rtt' : W[Γ ||-<l> t ≅ t' : tProd F G | RΠ]< wl >)
+  (Ru : W[Γ ||-<l'> u : F | RF]< wl >)
+  (Ru' : W[Γ ||-<l'> u' : F' | RF']< wl >)
+  (Ruu' : W[Γ ||-<l'> u ≅ u' : F | RF ]< wl >)
+  (RGu : W[Γ ||-<l'> X]< wl >)
+   : X = G[u..] ->
+    W[Γ ||-<l'> tApp t u ≅ tApp t' u' : X | RGu]< wl >.
+Proof.
+  intros eq.
+  eapply WLRTmEqIrrelevant' ; [symmetry; apply eq|].
+  eapply WappcongTerm; tea.
+  eapply WLRTmRedConv ; tea.
+  now eapply WLRTyEqSym.
+  Unshelve. now rewrite <- eq.
+Qed.
+
 End Application.
-
-
