theories/LogicalRelation/Monotonicity.v
@@ -1,127 +1,742 @@
-(** * LogRel.LogicalRelation.Escape: the logical relation implies conversion/typing. *)
-Require Import PeanoNat Nat.
-From Coq Require Import CRelationClasses.
 From LogRel.AutoSubst Require Import core unscoped Ast Extra.
-From LogRel Require Import Utils BasicAst Notations LContexts Context NormalForms GenericTyping LogicalRelation DeclarativeInstance.
-From LogRel.LogicalRelation Require Import Induction.
+From LogRel Require Import Notations Utils BasicAst LContexts Context NormalForms UntypedValues Weakening GenericTyping Monad LogicalRelation DeclarativeInstance.
+From LogRel.LogicalRelation Require Import Induction Irrelevance Reflexivity Transitivity Escape Weakening.
 
 Set Universe Polymorphism.
 
-Section Monotonicity.
+Section Red_Ltrans.
   Context `{GenericTypingProperties}.
-
-Lemma LRTy_Ltrans@{i i' j j' k k' l l'} {lA} (wl wl' : wfLCon) (f : wl' ≤ε wl)
-    (Γ : context) (A : term) :
-    [ LogRel@{i j k l} lA | Γ ||- A ]< wl > ->
-    [ LogRel@{i j k l} lA | Γ ||- A ]< wl' >.
+  
+Lemma Id_Ltrans@{h i j k l} (l : TypeLevel) (wl : wfLCon) (Γ : context) (A : term)
+  (IA : IdRedTy@{i j k l} wl Γ l A)
+  (ih1 : forall wl' : wfLCon,
+      wl' ≤ε wl -> [LogRel@{i j k l} l | Γ ||- IdRedTy.ty@{i j k l} IA ]< wl' >)
+  (ih2 : forall (Δ : context) (wl' : wfLCon) (ρ : Δ ≤ Γ),
+      wl' ≤ε wl -> [ |-[ ta ] Δ ]< wl' > ->
+      forall wl'' : wfLCon,
+        wl'' ≤ε wl' ->
+        [LogRel@{i j k l} l | Δ ||- (IdRedTy.ty@{i j k l} IA)⟨ρ⟩ ]< wl'' >)
+  (wl' : wfLCon)
+  (f : wl' ≤ε wl)
+  (Hg : [ |-[ ta ] Γ ]< wl >) : IdRedTy@{i j k l} wl' Γ l A.
 Proof.
-  intros [ [] lrA ] ; cbn in lrA.
-  induction lrA as [? ? ? [l1 lt1] | ? ? ? [] | ? ? ? [] [] IHdom IHcod|??? []|??? [] |??? []] ; intros.
-  - unshelve eapply LRU_.
-    unshelve econstructor ; try assumption.
-    + now eapply wfc_Ltrans.
-    + destruct red.
-      split ; try now eapply redty_Ltrans.
-      now eapply wft_Ltrans.
-  - unshelve eapply LRne_.
-    unshelve econstructor ; try assumption.
-    + destruct red ; split ; try now eapply redty_Ltrans.
-      now eapply wft_Ltrans.
-    + now eapply ty_ne_Ltrans.
+  unshelve econstructor.
+  6: econstructor ; [eapply wft_Ltrans, (IdRedTy.red IA).(tyr_wf_r _ _ _ _) ; eauto |
+                      eapply redty_Ltrans ; eauto].
+  3: now eapply (IdRedTy.red IA).(tyr_wf_red _ _ _ _).
+  3: eapply convty_Ltrans ; eauto ; now eapply (IdRedTy.eq IA).
+  + now eapply ih1.
+  + intros * f' Hd ; eapply ih2 ; [ | eassumption | now eapply wfLCon_le_id].
+    now eapply wfLCon_le_trans.
+  + irrelevance0 ; [ now eapply (wk_id_ren_on Γ (IdRedTy.ty IA)) | ].
+    destruct (wk_id_ren_on Γ  (IdRedTy.lhs IA)). 
+    eapply (IdRedTy.tyKripkeTm IA wk_id _ _ (wfLCon_le_id _) f Hg (wfc_Ltrans f Hg)).
+    * now bsimpl.
+    * irrelevance0 ; [symmetry ; now eapply (wk_id_ren_on Γ (IdRedTy.ty IA)) | ].
+      now eapply (IdRedTy.lhsRed).
+  + irrelevance0 ; [ now eapply (wk_id_ren_on Γ (IdRedTy.ty IA)) | ].
+    destruct (wk_id_ren_on Γ  (IdRedTy.rhs IA)).
+    eapply (IdRedTy.tyKripkeTm IA wk_id _ _ (wfLCon_le_id _) f Hg (wfc_Ltrans f Hg)).
+    * now bsimpl.
+    * irrelevance0 ; [symmetry ; now eapply (wk_id_ren_on Γ (IdRedTy.ty IA)) | ].
+      now eapply (IdRedTy.rhsRed).
+  + irrelevance0 ; [ now eapply (wk_id_ren_on Γ (IdRedTy.ty IA)) | ].
+    destruct (wk_id_ren_on Γ  (IdRedTy.lhs IA)).
+    eapply (IdRedTy.tyKripkeTmEq IA wk_id _ _ (wfLCon_le_id _) f Hg (wfc_Ltrans f Hg)).
+    * now bsimpl.
+    * irrelevance0 ; [symmetry ; now eapply (wk_id_ren_on Γ (IdRedTy.ty IA)) | ].
+      now eapply (IdRedTy.lhsRedRefl).
+  + irrelevance0 ; [ now eapply (wk_id_ren_on Γ (IdRedTy.ty IA)) | ].
+    destruct (wk_id_ren_on Γ  (IdRedTy.rhs IA)).
+    eapply (IdRedTy.tyKripkeTmEq IA wk_id _ _ (wfLCon_le_id _) f Hg (wfc_Ltrans f Hg)).
+    * now bsimpl.
+    * irrelevance0 ; [symmetry ; now eapply (wk_id_ren_on Γ (IdRedTy.ty IA)) | ].
+      now eapply (IdRedTy.rhsRedRefl).
+  + econstructor.
+    * intros ??? ; eapply (LREqTermSymConv); [eassumption | ].
+      now eapply reflLRTyEq.
+    * intros ????? ; eapply (transEqTerm@{h i j k l}) ; eassumption.
+  + intros ?? wl'' wl''' ??? f' f'' ??? Heq Hyp.
+    irrelevance0 ; [reflexivity | ].
+    eapply (IdRedTy.tyKripkeEq IA _ _ _ (f' •ε f) f'' wfΔ wfΞ _ Heq).
+    irrelevance0 ; [ reflexivity | eassumption].
+  + intros ?? wl'' wl''' ??? f' f'' ??? Heq Hyp.
+    irrelevance0 ; [reflexivity | ].
+    eapply (IdRedTy.tyKripkeTm IA _ _ _ (f' •ε f) f'' wfΔ wfΞ _ Heq).
+    irrelevance0 ; [ reflexivity | eassumption].
+  + intros ?? wl'' wl''' ??? f' f'' ???? Heq Hyp.
+    irrelevance0 ; [reflexivity | ].
+    eapply (IdRedTy.tyKripkeTmEq IA _ _ _ (f' •ε f) f'' wfΔ wfΞ _ _ Heq).
+    irrelevance0 ; [ reflexivity | eassumption].
+Defined.
+
+  Lemma Ltrans@{h i j k l} {wl Γ wl' A l} :
+    (wl' ≤ε wl) ->
+    [LogRel@{i j k l} l | Γ ||- A]< wl > ->
+    [LogRel@{i j k l} l | Γ ||- A]< wl' >.
+  Proof.
+    intros f lrA. revert wl' f. pattern l, wl, Γ, A, lrA.
+    eapply LR_rect_TyUr@{i j k l l}; clear l wl Γ A lrA.
+    - intros * [??? []] ??. apply LRU_.
+      econstructor ; eauto ; [now eapply wfc_Ltrans | econstructor ].
+      + now eapply wft_Ltrans.
+      + now eapply redty_Ltrans.
+    - intros ????[ty[]]??. apply LRne_ ; econstructor ; [econstructor | ].
+      + now eapply wft_Ltrans.
+      + now eapply redty_Ltrans.
+      + now eapply convneu_Ltrans.
+    - intros ???? [] ihdom ihcod wl' f ; cbn in *.
+      apply LRPi' ; econstructor ; [destruct red ; econstructor |..].
+      + now eapply wft_Ltrans.
+      + now eapply redty_Ltrans.
+      + now eapply convty_Ltrans.
+      + now eapply convty_Ltrans.
+      + unshelve econstructor.
+        4,5: destruct polyRed ; now eapply wft_Ltrans.
+        * intros * f' Hd.
+          eapply (PolyRed.shpRed polyRed) ; [eapply wfLCon_le_trans | ] ; eauto.
+        * intros ???? f' Hd ha ; cbn in *.
+          eapply (PolyRed.posTree polyRed) ; eauto.
+        * intros ???? f' ??? Hover ; cbn in *.
+          eapply (PolyRed.posRed polyRed) ; eassumption.
+        * intros ???? f' ????? Hover Hover' ; cbn in *.
+          eapply (PolyRed.posExt polyRed) ; eassumption.
+    - intros ????? wl' f.
+      eapply LRNat_ ; econstructor.
+      eapply redtywf_Ltrans ; eauto.
+      now eapply NA.(NatRedTy.red).
+    - intros ????? wl' f.
+      eapply LRBool_ ; econstructor.
+      eapply redtywf_Ltrans ; eauto.
+      now eapply NA.(BoolRedTy.red).
+    - intros ????? wl' f.
+      eapply LREmpty_ ; econstructor.
+      eapply redtywf_Ltrans ; eauto.
+      now eapply NA.(EmptyRedTy.red).
+    - intros ???? [] ihdom ihcod wl' f ; cbn in *.
+      apply (LRSig'@{i j k l}) ; econstructor ; [destruct red ; econstructor |..].
+      + now eapply wft_Ltrans.
+      + now eapply redty_Ltrans.
+      + now eapply convty_Ltrans.
+      + now eapply convty_Ltrans.
+      + unshelve econstructor.
+        4,5: destruct polyRed ; now eapply wft_Ltrans.
+        * intros * f' Hd.
+          eapply (PolyRed.shpRed polyRed) ; [eapply wfLCon_le_trans | ] ; eauto.
+        * intros ???? f' Hd ha ; cbn in *.
+          eapply (PolyRed.posTree polyRed) ; eauto.
+        * intros ???? f' ??? Hover ; cbn in *.
+          eapply (PolyRed.posRed polyRed) ; eassumption.
+        * intros ???? f' ????? Hover Hover' ; cbn in *.
+          eapply (PolyRed.posExt polyRed) ; eassumption.
+    - intros ????? ih1 ih2 wl' f. 
+      apply (LRId'@{i j k l}).
+      eapply (Id_Ltrans@{h i j k l}) ; eauto.
+      now eapply (wfc_convty (IdRedTy.eq IA)).
+  Defined.
+
+  Lemma WLtrans@{h i j k l} {wl Γ wl' A l} :
+    (wl' ≤ε wl) ->
+    WLogRel@{i j k l} l wl Γ A  ->
+    WLogRel@{i j k l} l wl' Γ A.
+  Proof.
+    intros f HA ; unshelve econstructor.
+    - eapply DTree_Ltrans ; [eassumption | ].
+      exact (WT _ HA).
+    - intros wl'' Hover.
+      eapply (WRed _ HA).
+      now eapply over_tree_Ltrans.
+  Defined.      
+
+  
+Lemma Eq_Ltrans@{h i j k l} {wl Γ wl' A B l} (f : wl' ≤ε wl) (lrA : [Γ ||-<l> A]< wl >) : 
+    [LogRel@{i j k l} l | Γ ||- A ≅ B | lrA]< wl > ->
+    [LogRel@{i j k l} l | Γ ||- A ≅ B | Ltrans@{h i j k l} f lrA]< wl' >.
+Proof.
+  revert B wl' f. pattern l, wl, Γ, A, lrA.
+  eapply LR_rect_TyUr@{i j k l l}; clear l wl Γ A lrA.
+  - intros ???? [??? []] ???[] ; cbn in *.
+    constructor ; constructor.
+    + now eapply wft_Ltrans.
+    + destruct red ; now eapply redty_Ltrans.
+  - intros ???? [?[]] ???[?[]] ; cbn in *.
+    econstructor ; [econstructor | ].
+    + now eapply wft_Ltrans.
+    + now eapply redty_Ltrans.
     + now eapply convneu_Ltrans.
-  - unshelve eapply LRPi_.
-    cbn in *.
-    unshelve econstructor.
-    + exact dom.
-    + exact cod.
-    + exact domN.
-    + intros.
-      unshelve eapply domRed ; try assumption.
-      now eapply wfLCon_le_trans.
-    + intros.
-      unshelve eapply codomN ; try assumption.
-      now eapply wfLCon_le_trans.
-      assumption.
-    + intros ; cbn in *.
-      unshelve eapply codRed ; [ exact l' | ..] ; try assumption.
-      * now eapply wfLCon_le_trans.
-      * assumption.
-      * assumption.
-    + destruct red.
-      split.
-      2: unshelve eapply redty_Ltrans ; try assumption.
-      now eapply wft_Ltrans.
+  - intros ???? [] ihdom ihcod B wl' f []; cbn in *.
+    econstructor ; [destruct red0 ; econstructor |..].
     + now eapply wft_Ltrans.
-    + now eapply wft_Ltrans.
+    + now eapply redty_Ltrans.
     + now eapply convty_Ltrans.
-    + intros ; now eapply codExt.
-    + cbn in *.
-      econstructor.
-      * intros. now eapply domAd.
-      * intros. now eapply codAd.
-  - unshelve eapply LRNat_.
-    econstructor.
-    destruct red.
-    split ; try now eapply redty_Ltrans.
-    now eapply wft_Ltrans.
-  - unshelve eapply LRBool_.
-    destruct red.
-    econstructor.
-    split ; try now eapply redty_Ltrans.
-    now eapply wft_Ltrans.
-  - unshelve eapply LREmpty_.
-    destruct red.
-    econstructor.
-    split ; try now eapply redty_Ltrans.
-    now eapply wft_Ltrans.
+    + now eapply convty_Ltrans.
+    + unshelve econstructor ; cbn in *.
+      * intros * ? ; now eapply (PolyRedEq.posTree polyRed0).
+      * intros * ; now eapply (PolyRedEq.shpRed polyRed0).
+      * cbn ; intros * Ho' ; now eapply (PolyRedEq.posRed polyRed0).
+  - intros ???? [[]] B wl' f [[]] ; cbn in *.
+    econstructor ; econstructor.
+    + now eapply wft_Ltrans.
+    + now eapply redty_Ltrans.
+  - intros ???? [[]] B wl' f [[]] ; cbn in *.
+    econstructor ; econstructor.
+    + now eapply wft_Ltrans.
+    + now eapply redty_Ltrans.
+  - intros ???? [[]] B wl' f [[]] ; cbn in *.
+    econstructor ; econstructor.
+    + now eapply wft_Ltrans.
+    + now eapply redty_Ltrans.
+  - intros ???? [] ihdom ihcod B wl' f [] ; cbn in *.
+    econstructor ; [destruct red0 ; econstructor | ..].
+    + now eapply wft_Ltrans.
+    + now eapply redty_Ltrans.
+    + now eapply convty_Ltrans.
+    + now eapply convty_Ltrans.
+    + unshelve econstructor ; cbn.
+      * intros * ? ; now eapply (PolyRedEq.posTree polyRed0).
+      * intros * ; now eapply (PolyRedEq.shpRed polyRed0).
+      * cbn ; intros * Ho' ; now eapply (PolyRedEq.posRed polyRed0).
+  - intros ????? ih1 ih2 ????.
+    assert (Hg:= (wfc_convty (IdRedTy.eq IA))).
+    eapply (@Build_IdRedTyEq _ _ _ _ _ _ wl' Γ A _ B) ; cbn.
+    + unshelve econstructor.
+      * now eapply wft_Ltrans, (IdRedTyEq.red X).(tyr_wf_r _ _ _ _).
+      * now eapply redty_Ltrans, (IdRedTyEq.red X).(tyr_wf_red _ _ _ _).
+    + eapply convty_Ltrans ; [ eassumption | ].
+      eapply (IdRedTyEq.eq X). 
+    + eapply ih1.
+      now eapply (IdRedTyEq.tyRed X).
+    + irrelevance0 ; [ now eapply (wk_id_ren_on Γ (IdRedTy.ty IA)) | ].
+      destruct (wk_id_ren_on Γ  (IdRedTy.lhs IA)).
+      destruct (wk_id_ren_on Γ  (IdRedTyEq.lhs X)).
+      eapply (IdRedTy.tyKripkeTmEq IA wk_id _ _ (wfLCon_le_id _) f Hg (wfc_Ltrans f Hg)).
+      * now bsimpl.
+      * irrelevance0 ; [ symmetry ; now eapply (wk_id_ren_on Γ (IdRedTy.ty IA)) | ].
+        exact (IdRedTyEq.lhsRed X).
+    + irrelevance0 ; [ now eapply (wk_id_ren_on Γ (IdRedTy.ty IA)) | ].
+      destruct (wk_id_ren_on Γ  (IdRedTy.rhs IA)).
+      destruct (wk_id_ren_on Γ  (IdRedTyEq.rhs X)).
+      eapply (IdRedTy.tyKripkeTmEq IA wk_id _ _ (wfLCon_le_id _) f Hg (wfc_Ltrans f Hg)).
+      * now bsimpl.
+      * irrelevance0 ; [ symmetry ; now eapply (wk_id_ren_on Γ (IdRedTy.ty IA)) | ].
+        exact (IdRedTyEq.rhsRed X).
 Qed.
 
-Lemma LRTyEq_Ltrans@{i j k l i' j' k' l'} lA lA'
-  (wl wl' : wfLCon) (f : wl' ≤ε wl) Γ A        
-  (lrA : [LogRel@{i j k l} lA | Γ ||- A]< wl >)
-  (lrA' : [LogRel@{i' j' k' l'} lA' | Γ ||- A]< wl' >) :
-  forall B, [Γ ||-< lA > A ≅ B | lrA]< wl > ->
-            [Γ ||-< lA' > A ≅ B | lrA']< wl' >.
-Admitted.
+  Lemma WEq_Ltrans@{h i j k l} {wl Γ wl' A B l}
+    (f : wl' ≤ε wl) (lrA : W[Γ ||-<l> A]< wl >) :
+    WLogRelEq@{i j k l} l wl Γ A B lrA ->
+    WLogRelEq@{i j k l} l wl' Γ A B (WLtrans@{h i j k l} f lrA).
+  Proof.
+    intros Heq ; unshelve econstructor.
+    - eapply DTree_Ltrans ; [eassumption | ].
+      exact (WTEq _ Heq).
+    - intros wl'' Hover Hover'.
+      eapply (WRedEq _ Heq).
+      now eapply over_tree_Ltrans.
+  Defined.      
 
 
-Lemma LRTm_Ltrans@{i j k l i' j' k' l'} lA lA'
-  (wl wl' : wfLCon) (f : wl' ≤ε wl) Γ A        
-  (lrA : [LogRel@{i j k l} lA | Γ ||- A]< wl >)
-  (lrA' : [LogRel@{i' j' k' l'} lA' | Γ ||- A]< wl' >) :
-  forall t, [Γ ||-< lA > t : A | lrA]< wl > ->
-            [Γ ||-< lA' > t : A | lrA']< wl' >.
-Admitted.
 
+Lemma isLRFun_Ltrans : forall wl wl' Γ t A l (f : wl' ≤ε wl) (ΠA : [Γ ||-Π< l > A]< wl >)
+                              (ΠA' : [Γ ||-Π< l > A]< wl' >),
+    isLRFun ΠA t -> isLRFun ΠA' t.
+Proof.
+  intros * f * Hyp.
+  unshelve epose (Heq := redtywf_det _ _ (redtywf_Ltrans f ΠA.(ParamRedTyPack.red)) ΠA'.(ParamRedTyPack.red)).
+  1,2: now econstructor.
+  inversion Heq.
+  induction Hyp as [?? funTree e r | t Heqt].
+  - unshelve econstructor.
+    + intros Δ wl'' a ρ f' Hd ha ; cbn.
+      eapply DTree_fusion.
+      * unshelve eapply funTree.
+        6: irrelevance0 ; [ | exact ha] ; now f_equal.
+        2: assumption.
+        now eapply wfLCon_le_trans.
+      * unshelve eapply (PolyRedPack.posTree ΠA).
+        5: eassumption.
+        4: irrelevance0 ; [ | exact ha] ; now f_equal.
+        now eapply wfLCon_le_trans.
+    + intros Δ wl'' ρ f' Hd ; cbn.
+      irrelevance0 ; [ | unshelve eapply e] ; [now f_equal | ..].
+      2: assumption.
+      now eapply wfLCon_le_trans.
+    + intros Δ wl'' a ρ f' Hd ha wl''' Ho Ho'.
+      irrelevance0 ; [ | unshelve eapply r].
+      now f_equal.
+      3: eassumption.
+      now eapply wfLCon_le_trans.
+      cbn in *.
+      3: now eapply over_tree_fusion_l.
+      now eapply over_tree_fusion_r.
+  - econstructor 2.
+    cbn in *.
+    rewrite <- H11, <- H12.
+    now eapply convneu_Ltrans.
+Qed.
 
-Lemma LRTm_Ltrans'@{i j k l i' j' k' l'} lA lA'
-  (wl wl' : wfLCon) (f : wl' ≤ε wl) Γ A        
-  (lrA : [LogRel@{i j k l} lA | Γ ||- A]< wl >)
-  (lrA' : [LogRel@{i' j' k' l'} lA' | Γ ||- A]< wl' >) :
-  forall t, [Γ ||-< lA > t : A | lrA]< wl > ->
-            [Γ ||-< lA' > t : A | lrA']< wl' >.
-Admitted.
+Lemma isLRPair_Ltrans : forall wl wl' Γ t A l (f : wl' ≤ε wl) (ΣA : [Γ ||-Σ< l > A]< wl >)
+                              (ΣA' : [Γ ||-Σ< l > A]< wl' >),
+    isLRPair ΣA t -> isLRPair ΣA' t.
+Proof.
+  intros * f * Hyp.
+  unshelve epose (Heq := redtywf_det _ _ (redtywf_Ltrans f ΣA.(ParamRedTyPack.red)) ΣA'.(ParamRedTyPack.red)).
+  1,2: now econstructor.
+  inversion Heq.
+  induction Hyp as [????? fstTree ?? sndTree | t Heqt].
+  - unshelve econstructor.
+    + intros Δ wl'' a' ρ f' Hd ha ; cbn.
+      eapply DTree_fusion.
+      * unshelve eapply fstTree.
+        6: irrelevance0 ; [ | exact ha] ; now f_equal.
+        2: assumption.
+        now eapply wfLCon_le_trans.
+      * unshelve eapply (PolyRedPack.posTree ΣA).
+        5: eassumption.
+        4: irrelevance0 ; [ | exact ha] ; now f_equal.
+        now eapply wfLCon_le_trans.
+    + intros Δ wl'' ρ f' Hd ; cbn.
+      irrelevance0 ; [ | unshelve eapply rfst] ; [now f_equal | ..].
+      2: assumption.
+      now eapply wfLCon_le_trans.
+    + intros Δ wl'' ρ f' Hd.
+      eapply DTree_fusion.
+      * eapply sndTree.
+        1,3: eassumption.
+        now eapply wfLCon_le_trans.
+      * unshelve  eapply (PolyRed.posTree ΣA).
+        6: now unshelve eapply rfst.
+        2,4: eassumption.
+        now eapply wfLCon_le_trans.
+    + intros Δ wl'' ρ f' Hd.
+      irrelevance0 ; [ | unshelve eapply rdom ; eauto].
+      now f_equal.
+      now eapply wfLCon_le_trans.
+    + intros Δ wl'' a' ρ f' Hd ha wl''' Ho Ho' ; cbn in *.
+      irrelevance0 ; [ | unshelve eapply rcod].
+      1: now f_equal.
+      3: eassumption.
+      * now eapply wfLCon_le_trans.
+      * irrelevance0 ; [ | exact ha] ; now f_equal.
+      * cbn in * ; now eapply over_tree_fusion_r.
+      * cbn in * ; now eapply over_tree_fusion_l.
+    + intros Δ wl'' ρ f' Hd wl''' Ho Ho' ; cbn in *.
+      irrelevance0 ; [ | unshelve eapply rsnd].
+      1: now f_equal.
+      3: eassumption.
+      * now eapply wfLCon_le_trans.
+      * cbn in * ; now eapply over_tree_fusion_r.
+      * cbn in * ; now eapply over_tree_fusion_l.
+  - econstructor 2.
+    cbn in *.
+    rewrite <- H11, <- H12.
+    now eapply convneu_Ltrans.
+Qed.
 
+Lemma NatTm_Ltrans (l : TypeLevel) (wl : wfLCon) (Γ : context) (A : term)
+  (NA : [Γ ||-Nat A ]< wl >) (t : term) (wl' : wfLCon) (f : wl' ≤ε wl) (NA' : [Γ ||-Nat A ]< wl' >) :
+  [LRNat_ l NA | Γ ||- t : A ]< wl > -> [ (LRNat_ l NA') | Γ ||- t : A ]< wl' >.
+Proof.
+  revert t.
+  set (G := _); enough (h : G × (forall t, NatProp NA t -> NatProp NA' t)) by apply h.
+  subst G; apply NatRedInduction.
+  - intros t nf Hred Heq Hprop Hprop'.
+    econstructor ; [now eapply redtmwf_Ltrans | | ].
+    + now eapply convtm_Ltrans.
+    + assumption.
+  - now econstructor.
+  - intros n Hn Hn' ; now econstructor.
+  - intros ; econstructor.
+    destruct r ; econstructor.
+    + now eapply ty_Ltrans.
+    + now eapply convneu_Ltrans.
+Qed.
 
-Lemma LRTmEq_Ltrans@{i j k l i' j' k' l'} lA lA'
-  (wl wl' : wfLCon) (f : wl' ≤ε wl) Γ A        
-  (lrA : [LogRel@{i j k l} lA | Γ ||- A]< wl >)
-  (lrA' : [LogRel@{i' j' k' l'} lA' | Γ ||- A]< wl' >) :
-  forall t u, [Γ ||-< lA > t ≅ u : A | lrA]< wl > ->
-            [Γ ||-< lA' > t ≅ u : A | lrA']< wl' >.
-Admitted.
-(*  intros B eqB.
-  destruct lrA as [ [] lrA] ; cbn in *.
-  induction lrA.
+Lemma IdTm_Ltrans (l : TypeLevel) (wl wl' : wfLCon) (Γ : context) (A : term) (f : wl' ≤ε wl)
+  (IA : [Γ ||-Id< l > A ]< wl >) (IA' : [Γ ||-Id< l > A ]< wl' >)
+  (ih1 : forall (t : term),
+      [IdRedTy.tyRed IA | Γ ||- t : IdRedTy.ty IA ]< wl > ->
+      [IdRedTy.tyRed IA' | Γ ||- t : IdRedTy.ty IA' ]< wl' >)
+  (ih2 : forall (Δ : context) (ρ : Δ ≤ Γ) (wfΔ : [ |-[ ta ] Δ ]< wl' >)
+                (t : term) (wl'' : wfLCon) (f' : wl'' ≤ε wl'),
+      [IdRedTy.tyKripke IA ρ f wfΔ | Δ ||- t : (IdRedTy.ty IA)⟨ρ⟩ ]< wl' > ->
+      [IdRedTy.tyKripke IA' ρ f' (wfc_Ltrans f' wfΔ) | Δ ||- t : (IdRedTy.ty IA')⟨ρ⟩ ]< wl'' >) :
+      forall (t : term),
+        [LRId' IA | Γ ||- t : A ]< wl > -> [LRId' IA' | Γ ||- t : A ]< wl' >.
+Proof.
+  intros t Ht.
+  unshelve epose (Heq := redtywf_det _ _ (redtywf_Ltrans f (IdRedTy.red IA))
+                           (IdRedTy.red IA')).
+  1,2 : now econstructor.
+  inversion Heq.
+  assert (Hg:= (wfc_convty (IdRedTy.eq IA))).
+  econstructor ; cbn.
+  - cbv in H11,H12,H13 ; cbv. 
+    rewrite <- H11, <- H12, <- H13.
+    now eapply redtmwf_Ltrans ; [ | eapply (IdRedTm.red Ht)].
+  - cbv in H11,H12,H13 ; cbv. 
+    rewrite <- H11, <- H12, <- H13.
+    now eapply convtm_Ltrans ; [ | eapply (IdRedTm.eq Ht)].
+  - destruct (IdRedTm.prop Ht).
+    + econstructor.
+      * now eapply wft_Ltrans.
+      * now eapply ty_Ltrans.
+      * irrelevance0 ; [ | unshelve eapply Eq_Ltrans].
+        5: eassumption.
+        all: assumption.
+      * assert (Help : IdRedTyPack.lhs (IdRedTy.toPack IA') = IdRedTyPack.lhs (IdRedTy.toPack IA)).
+        { now eauto. }
+        rewrite Help.
+        irrelevance0.
+        2:{ erewrite <- (wk_id_ren_on Γ (IdRedTyPack.lhs (IdRedTy.toPack IA))).
+            erewrite <- wk_id_ren_on.
+            eapply (IdRedTy.tyKripkeTmEq IA wk_id wk_id _ (wfLCon_le_id _) f Hg (wfc_Ltrans f Hg)).
+            * now bsimpl.
+            * irrelevance0 ; [rewrite wk_id_ren_on ; reflexivity | ].
+              eassumption.
+        }
+        rewrite H11 ; bsimpl.
+        reflexivity.
+      * assert (Help : IdRedTyPack.rhs (IdRedTy.toPack IA') = IdRedTyPack.rhs (IdRedTy.toPack IA)).
+        { now eauto. }
+        rewrite Help.
+        irrelevance0.
+        2:{ erewrite <- (wk_id_ren_on Γ (IdRedTyPack.rhs (IdRedTy.toPack IA))).
+            erewrite <- wk_id_ren_on.
+            eapply (IdRedTy.tyKripkeTmEq IA wk_id wk_id _ (wfLCon_le_id _) f Hg (wfc_Ltrans f Hg)).
+            * now bsimpl.
+            * irrelevance0 ; [rewrite wk_id_ren_on ; reflexivity | ].
+              eassumption.
+        }
+        rewrite H11 ; bsimpl.
+        reflexivity.
+    + econstructor.
+      destruct r ; econstructor.
+      * eapply ty_Ltrans ; [eassumption | ].
+        assert (Help : IdRedTyPack.outTy (IdRedTy.toPack IA') = IdRedTyPack.outTy (IdRedTy.toPack IA)) by eauto.
+        now rewrite Help.
+      * eapply convneu_Ltrans ; [eassumption | ].
+        assert (Help : IdRedTyPack.outTy (IdRedTy.toPack IA') = IdRedTyPack.outTy (IdRedTy.toPack IA)) by eauto.
+        now rewrite Help.
+Qed.
+
+Lemma ΠTm_Ltrans (l : TypeLevel) (wl wl' : wfLCon) (Γ : context) (f : wl' ≤ε wl) (A : term)
+  (ΠA : [Γ ||-Π< l > A ]< wl >)
+  (ΠA' : [Γ ||-Π< l > A ]< wl' >)
+  (ihdom : forall (Δ : context) (ρ : Δ ≤ Γ) (h : [ |-[ ta ] Δ ]< wl' >) (t : term)
+                  (wl'' : wfLCon) (f' : wl'' ≤ε wl'),
+      [PolyRed.shpRed ΠA ρ f h | Δ ||- t : (ParamRedTy.dom ΠA)⟨ρ⟩ ]< wl' > ->
+      [Ltrans f' (PolyRed.shpRed ΠA ρ f h) | Δ ||- t : (ParamRedTy.dom ΠA)⟨ρ⟩ ]< wl'' >)
+  (ihcod : forall (Δ : context) (a : term) (ρ : Δ ≤ Γ) (h : [ |-[ ta ] Δ ]< wl' >)
+                  (ha : [PolyRed.shpRed ΠA ρ f h | Δ ||- a : (ParamRedTy.dom ΠA)⟨ρ⟩ ]< wl' >)
+                  (wl'' : wfLCon) (Ho : over_tree wl' wl'' (PolyRed.posTree ΠA ρ f h ha))
+                  (t : term) (wl''' : wfLCon) (f'' : wl''' ≤ε wl''),
+      [PolyRed.posRed ΠA ρ f h ha Ho | Δ  ||- t : (ParamRedTy.cod ΠA)[a .: ρ >> tRel] ]< wl'' > ->
+      [Ltrans f'' (PolyRed.posRed ΠA ρ f h ha Ho) | Δ  ||- t : (ParamRedTy.cod ΠA)[a .: ρ >> tRel] ]< wl''' >) :
+  forall (t : term),
+    [Γ ||-Π t : A | ΠA ]< wl > ->  [Γ ||-Π t : A | ΠA' ]< wl' >.
+Proof.
+  intros t [].
+  unshelve econstructor ; [ | | eapply redtmwf_Ltrans ; eauto |..].
+  1: exact nf.
+  1:{ cbn in * ; intros.
+      eapply DTree_fusion.
+      * unshelve eapply appTree.
+        4: eapply wfLCon_le_trans.
+        3-6: eassumption.
+        2: irrelevance0 ; [ | eassumption ].
+        f_equal.
+        unshelve epose (Heq := redtywf_det _ _ (redtywf_Ltrans f ΠA.(ParamRedTyPack.red)) ΠA'.(ParamRedTyPack.red)) ; [now econstructor | now econstructor | ].
+        now inversion Heq.
+    * eapply (PolyRed.posTree ΠA ρ (f0 •ε f) Hd).
+      irrelevance0 ; [ | eassumption].
+      f_equal.
+      unshelve epose (Heq := redtywf_det _ _ (redtywf_Ltrans f ΠA.(ParamRedTyPack.red)) ΠA'.(ParamRedTyPack.red)) ; [now econstructor | now econstructor | ].
+      now inversion Heq.
+  }
+  all: unshelve epose (Heq := redtywf_det _ _ (redtywf_Ltrans f ΠA.(ParamRedTyPack.red)) ΠA'.(ParamRedTyPack.red)) ; [now econstructor | now econstructor | ].
+  all: inversion Heq.
+  2: eapply convtm_Ltrans ; [eauto | now rewrite <- Heq].
+  2: eapply isLRFun_Ltrans ; eauto.
+  1: now rewrite <- Heq.
+  + cbn in * ; intros. 
+    irrelevance0 ; [ | unshelve eapply app].
+    6: now eapply over_tree_fusion_r.
+    * now f_equal.
+    * now eapply over_tree_fusion_l.
+  + cbn in * ; intros.
+    irrelevance0 ; [ | unshelve eapply eq].
+    9: now eapply over_tree_fusion_l.
+    2: now eapply over_tree_fusion_r.
+    1: now f_equal.
+    1,2: irrelevance0 ; [ | eassumption] ; now f_equal.
+Defined.
+
+Lemma ΣTm_Ltrans (l : TypeLevel) (wl wl' : wfLCon) (Γ : context) (f : wl' ≤ε wl) (A : term)
+  (ΣA : [Γ ||-Σ< l > A ]< wl >)
+  (ΣA' : [Γ ||-Σ< l > A ]< wl' >)
+  (ihdom : forall (Δ : context) (ρ : Δ ≤ Γ) (h : [ |-[ ta ] Δ ]< wl' >) (t : term)
+                  (wl'' : wfLCon) (f' : wl'' ≤ε wl'),
+      [PolyRed.shpRed ΣA ρ f h | Δ ||- t : (ParamRedTy.dom ΣA)⟨ρ⟩ ]< wl' > ->
+      [Ltrans f' (PolyRed.shpRed ΣA ρ f h) | Δ ||- t : (ParamRedTy.dom ΣA)⟨ρ⟩ ]< wl'' >)
+  (ihcod : forall (Δ : context) (a : term) (ρ : Δ ≤ Γ) (h : [ |-[ ta ] Δ ]< wl' >)
+                  (ha : [PolyRed.shpRed ΣA ρ f h | Δ ||- a : (ParamRedTy.dom ΣA)⟨ρ⟩ ]< wl' >)
+                  (wl'' : wfLCon) (Ho : over_tree wl' wl'' (PolyRed.posTree ΣA ρ f h ha))
+                  (t : term) (wl''' : wfLCon) (f'' : wl''' ≤ε wl''),
+      [PolyRed.posRed ΣA ρ f h ha Ho | Δ  ||- t : (ParamRedTy.cod ΣA)[a .: ρ >> tRel] ]< wl'' > ->
+      [Ltrans f'' (PolyRed.posRed ΣA ρ f h ha Ho) | Δ  ||- t : (ParamRedTy.cod ΣA)[a .: ρ >> tRel] ]< wl''' >) :
+  forall (t : term),
+    [Γ ||-Σ t : A | ΣA ]< wl > ->  [Γ ||-Σ t : A | ΣA' ]< wl' >.
+Proof.
+  intros t [].
+  unshelve econstructor.
+  4: eapply redtmwf_Ltrans ; eauto.
+  1: exact nf.
+  2:{ cbn in * ; intros.
+      eapply DTree_fusion.
+      * unshelve eapply sndTree.
+        3: eapply wfLCon_le_trans.
+        2-5: eassumption.
+      * eapply (PolyRed.posTree ΣA ρ (f0 •ε f) Hd).
+        eapply fstRed.
+  }
+  all: unshelve epose (Heq := redtywf_det _ _ (redtywf_Ltrans f ΣA.(ParamRedTyPack.red)) ΣA'.(ParamRedTyPack.red)) ; [now econstructor | now econstructor | ].
+  all: inversion Heq.
+  3: eapply convtm_Ltrans ; [eauto | ].
+  2,3: cbv ; cbv in Heq ; now rewrite <- Heq.
+  2: eapply isLRPair_Ltrans ; now eauto.
+  + cbn in * ; intros.
+    irrelevance0 ; [ | unshelve eapply fstRed].
+    * now f_equal.
+    * now eapply wfLCon_le_trans.
+    * assumption.
+  + cbn in * ; intros.
+    irrelevance0 ; [ | unshelve eapply sndRed].
+    4: eassumption.
+    * now f_equal.
+    * now eapply wfLCon_le_trans.
+    * now eapply over_tree_fusion_r.
+    * now eapply over_tree_fusion_l.
+Defined.
   
-  cbn.
-  induction lrA as [? ? ? ? | ? | ? ? A [] [] IHdom IHcod|?? NEA|?? NEA |?? NEA].
-  - cbn.
-    unshelve eapply LRTyEqIrrelevantCum ; [exact lA |..].
-    + eapply LRTy_Ltrans ; try eassumption.
-      eapply LRU_ ; econstructor ; eassumption.
-    + cbn.
-  pattern lA, wl, Γ, A, lrA. apply LR_rect_TyUr. clear lA Γ A lrA.
-*)
+Lemma Tm_Ltrans@{h i j k l} {wl Γ wl' t A l} (f : wl' ≤ε wl) (lrA : [Γ ||-<l> A]< wl >) : 
+    [LogRel@{i j k l} l | Γ ||- t : A | lrA]< wl > ->
+    [LogRel@{i j k l} l | Γ ||- t : A | Ltrans@{h i j k l} f lrA]< wl' >.
+Proof.
+  revert t wl' f. pattern l, wl, Γ, A, lrA.
+  eapply LR_rect_TyUr@{i j k l l}; clear l wl Γ A lrA.
+  - intros ???? [??? []] ???[?[]].
+    econstructor ; [ econstructor | eassumption |.. ].
+    + now eapply ty_Ltrans.
+    + now eapply redtm_Ltrans.
+    + now eapply convtm_Ltrans.
+    + apply RedTyRecBwd ; apply RedTyRecFwd in rel.
+      now eapply Ltrans ; eauto.
+  - intros ???? [?[]] ???[?[]] ; cbn in *.
+    econstructor ; [econstructor ; cbn | ].
+    + now eapply ty_Ltrans.
+    + now eapply redtm_Ltrans.
+    + now eapply convneu_Ltrans.
+  - intros ???? [] ihdom ihcod t wl' f ?.
+    cbn in *.
+    unshelve eapply ΠTm_Ltrans ; intros.
+    6: eassumption.
+    1: eassumption.
+    + now eapply ihdom.
+    + now eapply ihcod. 
+  - intros ; irrelevance0 ; [ reflexivity | unshelve eapply NatTm_Ltrans].
+    5: eassumption.
+    2: assumption.
+    destruct NA ; econstructor ; now eapply redtywf_Ltrans.
+  - intros ???? NA t ? f ; revert t ; cbn.
+    intros t Ht. induction Ht. econstructor.
+    + now eapply redtmwf_Ltrans.
+    + now eapply convtm_Ltrans.
+    + destruct prop as [ | | m Hne] ; econstructor.
+      destruct Hne ; econstructor.
+      * now eapply ty_Ltrans.
+      * now eapply convneu_Ltrans.
+  - intros ???? NA t ? f Ht ; cbn.
+    induction Ht ; econstructor.
+    + now eapply redtmwf_Ltrans.
+    + now eapply convtm_Ltrans.
+    + destruct prop as [m Hne] ; econstructor.
+      destruct Hne ; econstructor.
+      * now eapply ty_Ltrans.
+      * now eapply convneu_Ltrans.
+  - intros ????? ihdom ihcod t wl' f ?; cbn in *.
+    eapply ΣTm_Ltrans.
+    + intros ; eauto.
+    + intros ; eauto.
+    + assumption.
+      Unshelve. assumption.
+  - intros * ih1 ih2 *.
+    unshelve eapply IdTm_Ltrans.
+    eassumption.
+    + intros ; eapply ih1 ; auto.
+    + intros ; eapply ih2.
+      rewrite <- (wk_id_ren_on Δ t0).
+      eapply (IdRedTy.tyKripkeTm IA ρ).
+      * now bsimpl.
+      * eassumption.
+Qed.
 
-End Monotonicity.
+Lemma WTm_Ltrans@{h i j k l} {wl Γ wl' A t l}
+    (f : wl' ≤ε wl) (lrA : W[Γ ||-<l> A]< wl >) :
+    WLogRelTm@{i j k l} l wl Γ t A lrA ->
+    WLogRelTm@{i j k l} l wl' Γ t A (WLtrans@{h i j k l} f lrA).
+  Proof.
+    intros Ht ; unshelve econstructor.
+    - eapply DTree_Ltrans ; [eassumption | ].
+      exact (WTTm _ Ht).
+    - intros wl'' Hover Hover'.
+      eapply (WRedTm _ Ht).
+      now eapply over_tree_Ltrans.
+  Defined. 
+
+Lemma TmEq_Ltrans@{h i j k l} {wl Γ wl' t u A l} (f : wl' ≤ε wl) (lrA : [Γ ||-<l> A]< wl >) : 
+    [LogRel@{i j k l} l | Γ ||- t ≅ u : A | lrA]< wl > ->
+    [LogRel@{i j k l} l | Γ ||- t ≅ u : A | Ltrans@{h i j k l} f lrA]< wl' >.
+Proof.
+  revert t u wl' f. pattern l, wl, Γ, A, lrA.
+  eapply LR_rect_TyUr@{i j k l l}; clear l wl Γ A lrA.
+  - intros ???? [??? []] ???? [].
+    unshelve econstructor.
+    + destruct redL.
+      econstructor.
+      * now eapply redtmwf_Ltrans.
+      * assumption.
+      * now eapply convtm_Ltrans.
+      * apply RedTyRecBwd ; clear relEq ; apply RedTyRecFwd in relL.
+        now eapply Ltrans.
+    + destruct redR.
+      econstructor.
+      * now eapply redtmwf_Ltrans.
+      * assumption.
+      * now eapply convtm_Ltrans.
+      * apply RedTyRecBwd ; clear relEq ; apply RedTyRecFwd in relR.
+        now eapply Ltrans.
+    + apply RedTyRecBwd ; clear relEq ; apply RedTyRecFwd in relL.
+      now eapply Ltrans.
+    + cbn in *.
+      now eapply convtm_Ltrans.
+    + apply RedTyRecBwd ; clear relEq ; apply RedTyRecFwd in relR.
+      now eapply Ltrans.
+    + eapply TyEqRecBwd, Eq_Ltrans ; cbn.
+      now eapply TyEqRecFwd.
+  - intros ???? [?[]] ???? [] ; cbn in *.
+    econstructor.
+    + now eapply redtmwf_Ltrans.
+    + now eapply redtmwf_Ltrans.
+    + now eapply convneu_Ltrans.
+  - intros ????? ihdom ihcod t u wl' f [].
+    cbn.
+    unshelve econstructor ; cbn in *.
+    + unshelve eapply ΠTm_Ltrans ; [ | eassumption | ..].
+      1,4: eassumption.
+      * intros ; now eapply Tm_Ltrans.
+      * intros ; now eapply Tm_Ltrans.
+    + unshelve eapply ΠTm_Ltrans ; [ | eassumption | ..].
+      1,4: eassumption.
+      * intros ; now eapply Tm_Ltrans.
+      * intros ; now eapply Tm_Ltrans.
+    + intros ; eapply eqTree.
+      eassumption.
+    + intros ; cbn in *.
+      now eapply convtm_Ltrans.
+    + intros ; cbn in *.
+      eapply eqApp.
+      assumption.
+  - intros * ; revert t u.
+    set (NA' := {| NatRedTy.red := redtywf_Ltrans f (NatRedTy.red NA) |}).
+    set (G := _); enough (h : G × (forall t u, NatPropEq NA t u -> NatPropEq NA' t u)) by apply h.
+    subst G; apply NatRedEqInduction.
+    + intros t u nt nu Hredt Hredu Heq Hprop Hprop'.
+      econstructor.
+      1,2: now eapply redtmwf_Ltrans.
+      * now eapply convtm_Ltrans.
+      * assumption.
+    + now econstructor.
+    + intros n Hn Hn' ; now econstructor.
+    + intros ; econstructor.
+      destruct r ; econstructor.
+      now eapply convneu_Ltrans.
+  - intros ???? NA t ? wl' f Heq.
+    induction Heq ; cbn. econstructor.
+    1,2: now eapply redtmwf_Ltrans.
+    + now eapply convtm_Ltrans.
+    + destruct prop as [ | | m Hne] ; econstructor.
+      econstructor.
+      now destruct r ; eapply convneu_Ltrans.
+  - intros ???? NA t u wl' f Heq ; cbn.
+    induction Heq ; econstructor.
+    1,2: now eapply redtmwf_Ltrans.
+    + now eapply convtm_Ltrans.
+    + destruct prop as [m Hne] ; econstructor ; econstructor.
+      now destruct r ; eapply convneu_Ltrans.
+  - cbn ; intros ????? ihdom ihcod t u wl' f []; cbn in *.
+    unshelve econstructor ; cbn.
+    + unshelve eapply ΣTm_Ltrans.
+      2,3,6: eassumption.
+      * intros.
+        irrelevance0 ; [ | unshelve eapply Tm_Ltrans].
+        5: eassumption.
+        1,2: now auto.
+      * intros.
+        irrelevance0 ; [ | unshelve eapply Tm_Ltrans].
+        5: eassumption.
+        1,2: now trivial.
+    + unshelve eapply ΣTm_Ltrans.
+      2,3,6: eassumption.
+      * intros.
+        irrelevance0 ; [ | unshelve eapply Tm_Ltrans].
+        5: eassumption.
+        1,2: now auto.
+      * intros.
+        irrelevance0 ; [ | unshelve eapply Tm_Ltrans].
+        5: eassumption.
+        1,2: now trivial.
+    + intros ; eapply DTree_fusion.
+      * eapply eqTree.
+        1,3: eassumption.
+        now eapply wfLCon_le_trans.
+      * eapply (PolyRed.posTree ΠA ρ (f0 •ε f) Hd).
+        now eapply (SigRedTm.fstRed redL). 
+    + cbn ; now eapply convtm_Ltrans.
+    + cbn ; intros ; now unshelve eapply eqFst.
+    + cbn in * ; intros.
+      irrelevance0 ; [ reflexivity | unshelve eapply eqSnd].
+      3: eassumption.
+      * now eapply wfLCon_le_trans.
+      * now eapply over_tree_fusion_r.
+      * now eapply over_tree_fusion_l.
+  - intros ????? ih1 ih2 ???? [].
+    unshelve econstructor ; cbn.
+    3,4: now eapply redtmwf_Ltrans.
+    1: now eapply convtm_Ltrans.
+    destruct prop.
+    + econstructor.
+      1,2: now eapply wft_Ltrans.
+      1,2: now eapply ty_Ltrans.
+      1,2:irrelevance0 ; [ | now eapply Eq_Ltrans] ; reflexivity.
+      all: now eapply ih1.
+    + econstructor.
+      destruct r ; econstructor.
+      now eapply convneu_Ltrans.
+      Unshelve. all: assumption.
+Qed.
+
+Lemma WTmEq_Ltrans@{h i j k l} {wl Γ wl' t u A l}
+    (f : wl' ≤ε wl) (lrA : W[Γ ||-<l> A]< wl >) :
+    WLogRelTmEq@{i j k l} l wl Γ t u A lrA ->
+    WLogRelTmEq@{i j k l} l wl' Γ t u A (WLtrans@{h i j k l} f lrA).
+  Proof.
+    intros Htu ; unshelve econstructor.
+    - eapply DTree_Ltrans ; [eassumption | ].
+      exact (WTTmEq _ Htu).
+    - intros wl'' Hover Hover'.
+      eapply (WRedTmEq _ Htu).
+      now eapply over_tree_Ltrans.
+  Defined. 
+
+End Red_Ltrans.
