theories/LogicalRelation/Reduction.v
@@ -1,6 +1,6 @@
 (* From Coq.Classes Require Import CRelationClasses. *)
 From LogRel.AutoSubst Require Import core unscoped Ast Extra.
-From LogRel Require Import Notations Utils BasicAst LContexts Context NormalForms UntypedReduction Weakening GenericTyping LogicalRelation DeclarativeInstance.
+From LogRel Require Import Notations Utils BasicAst LContexts Context NormalForms UntypedReduction Weakening GenericTyping Monad LogicalRelation DeclarativeInstance.
 From LogRel.LogicalRelation Require Import Induction Reflexivity Universe Escape Irrelevance.
 
 Set Universe Polymorphism.
@@ -12,7 +12,7 @@ Set Printing Primitive Projection Parameters.
 
 Lemma redSubst {wl Γ A B l} :
   [Γ ||-<l> B]< wl > ->
-  [Γ |- A ⇒* B]< wl > ->
+  [Γ |- A ⤳* B]< wl > ->
   ∑ (RA : [Γ ||-<l> A]< wl >), [Γ ||-<l> A ≅ B | RA]< wl >.
 Proof.
   intros RB; revert A; pattern l, wl, Γ, B, RB; apply LR_rect_TyUr; clear l wl Γ B RB; intros l wl Γ.
@@ -25,13 +25,12 @@ Proof.
       constructor; tea; gen_typing.
     + exists t; tea.
   - intros B [dom cod] A ? ihdom ihcod; cbn in *; unshelve eexists.
-    + apply LRPi'; unshelve eexists dom cod _ _ _ _; tea; etransitivity; tea.
+    + apply LRPi'; unshelve eexists dom cod ; tea; etransitivity; tea.
       constructor; tea; gen_typing.
-    + unshelve eexists dom cod _ _; tea; cbn.
-      2,3: intros; apply LRTyEqRefl_.
-      intros ; unshelve eapply codomN.
-      6: exact Ninfl.
-      all: try assumption.
+    + unshelve eexists dom cod ; tea; cbn.
+      unshelve econstructor;intros.
+      2,3: apply reflLRTyEq.
+      now eapply leaf.
   - intros B [red] A ?; unshelve eexists.
     + apply LRNat_; constructor; tea; etransitivity; tea.
       constructor; tea; gen_typing.
@@ -44,28 +43,39 @@ Proof.
     + apply LREmpty_; constructor; tea; etransitivity; tea.
       constructor; tea; gen_typing.
     + now constructor.
+  - intros B [dom cod] A ? ihdom ihcod; cbn in *; unshelve eexists.
+    + apply LRSig'; unshelve eexists dom cod; tea; etransitivity; tea.
+      constructor; tea; gen_typing.
+    + unshelve eexists dom cod; tea; cbn.
+      unshelve econstructor;intros; try now apply reflLRTyEq.
+      now eapply leaf.
+  - intros ? [ty lhs rhs] ih _ X redX; unshelve eexists.
+    + apply LRId'; unshelve eexists ty lhs rhs _ _; tea.
+      etransitivity; tea; constructor; tea; gen_typing.
+    + exists ty lhs rhs; tea; eapply reflLRTyEq.
 Qed.
 
 Lemma WredSubst {wl Γ A B l} :
   W[Γ ||-<l> B]< wl > ->
-  [Γ |- A ⇒* B]< wl > ->
+  [Γ |- A ⤳* B]< wl > ->
   ∑ (RA : W[Γ ||-<l> A]< wl >), W[Γ ||-<l> A ≅ B | RA]< wl >.
 Proof.
   intros [] ?.
   unshelve econstructor.
-  - exists WN.
+  - exists WT.
     intros.
     eapply redSubst.
     + eapply WRed ; try assumption.
-    + now eapply redty_Ltrans.
-  - exists WN.
+    + eapply redty_Ltrans ; eauto.
+      now eapply over_tree_le.
+  - exists WT.
     cbn ; intros.
-    now destruct (redSubst (WRed wl' τ Ninfl) (redty_Ltrans τ H14)).
+    now destruct (redSubst (WRed wl' Hover) (redty_Ltrans (over_tree_le Hover) H10)).
 Qed.   
     
 Lemma redwfSubst {wl Γ A B l} :
   [Γ ||-<l> B]< wl > ->
-  [Γ |- A :⇒*: B]< wl > ->
+  [Γ |- A :⤳*: B]< wl > ->
   ∑ (RA : [Γ ||-<l> A]< wl >), [Γ ||-<l> A ≅ B | RA]< wl >.
 Proof.
   intros ? []; now eapply redSubst.
@@ -73,14 +83,14 @@ Qed.
 
 Lemma redSubstTerm {wl Γ A t u l} (RA : [Γ ||-<l> A]< wl >) :
   [Γ ||-<l> u : A | RA]< wl > ->
-  [Γ |- t ⇒* u : A ]< wl > ->
+  [Γ |- t ⤳* u : A ]< wl > ->
   [Γ ||-<l> t : A | RA]< wl > × [Γ ||-<l> t ≅ u : A | RA]< wl >.
 Proof.
   revert t u; pattern l, wl, Γ, A, RA; apply LR_rect_TyUr; clear l wl Γ A RA; intros l wl Γ.
   - intros ? h ?? ru' redtu; pose (ru := ru'); destruct ru' as [T].
     assert [Γ |- A ≅ U]< wl > by (destruct h; gen_typing).
     assert [Γ |- t : U]< wl > by (eapply ty_conv; [gen_typing| now escape]).
-    assert (redtu' : [Γ |-[ ta ] t ⇒* u]< wl >) by gen_typing.
+    assert (redtu' : [Γ |-[ ta ] t ⤳* u]< wl >) by gen_typing.
     destruct (redSubst (A:=t) (RedTyRecFwd h rel) redtu') as [rTyt0].
     pose proof (rTyt := RedTyRecBwd h rTyt0).
     unshelve refine (let rt : [LRU_ h | Γ ||- t : A]< wl >:= _ in _).
@@ -93,30 +103,31 @@ Proof.
       destruct neA; cbn in *.
       eapply convty_exp.
        2: apply redtywf_refl; gen_typing.
-       2: apply convty_term; now apply convtm_convneu.
+       2: apply convty_term, convtm_convneu ; eauto.
        gen_typing.
+       now constructor.
     }
-    assert [Γ |-[ ta ] t ⇒* u : neRedTy.ty neA]< wl > by (eapply redtm_conv; tea). 
+    assert [Γ |-[ ta ] t ⤳* u : neRedTy.ty neA]< wl > by (eapply redtm_conv; tea). 
     assert [Γ |-[ ta ] t : neRedTy.ty neA]< wl > by (eapply ty_conv; tea; gen_typing). 
     unshelve refine (let rt : [LRne_ l neA | Γ ||- t : A]< wl > := _ in _).
     + exists n; tea; destruct red; constructor; tea; now etransitivity.
     + split; tea; exists n n; tea; destruct red; constructor; tea; now etransitivity. 
   - intros ? ΠA ihdom ihcod ?? ru' ?; pose (ru := ru'); destruct ru' as [f].
-    assert [Γ |- A ≅ PiRedTyPack.prod ΠA]< wl >. 1:{
+    assert [Γ |- A ≅ ΠA.(outTy)]< wl >. 1:{
       destruct ΠA as [?? []]. cbn in *.
       eapply convty_exp; tea.
       now apply redtywf_refl.
     }
-    assert [Γ |-[ ta ] t ⇒* u : PiRedTyPack.prod ΠA]< wl > by now eapply redtm_conv. 
-    assert [Γ |-[ ta ] t : PiRedTyPack.prod ΠA]< wl > by (eapply ty_conv; gen_typing).
+    assert [Γ |-[ ta ] t ⤳* u : ΠA.(outTy)]< wl > by now eapply redtm_conv. 
+    assert [Γ |-[ ta ] t : ΠA.(outTy)]< wl > by (eapply ty_conv; gen_typing).
     unshelve refine (let rt : [LRPi' ΠA | Γ ||- t : A]< wl > := _ in _).
-    1: exists f redN appN ; tea ; constructor ; destruct red ; tea ; etransitivity ; tea.
+    1: exists f appTree ; tea ; constructor ; destruct red ; tea ; etransitivity ; tea.
     split; tea; unshelve eexists ; tea.
     intros; cbn. eapply eq; tea.
-    now apply LREqTermRefl_.
+    now apply reflLRTmEq.
   - intros ? NA t ? Ru red; inversion Ru; subst.
     assert [Γ |- A ≅ tNat]< wl > by (destruct NA; gen_typing).
-    assert [Γ |- t :⇒*: nf : tNat]< wl >. 1:{
+    assert [Γ |- t :⤳*: nf : tNat]< wl >. 1:{
       constructor. 1: gen_typing.
       etransitivity. 2: gen_typing.
       now eapply redtm_conv.
@@ -125,7 +136,7 @@ Proof.
     now eapply reflNatRedTmEq.
   - intros ? NA t ? Ru red; inversion Ru; subst.
     assert [Γ |- A ≅ tBool]< wl > by (destruct NA; gen_typing).
-    assert [Γ |- t :⇒*: nf : tBool]< wl >. 1:{
+    assert [Γ |- t :⤳*: nf : tBool]< wl >. 1:{
       constructor. 
       1: eapply ty_conv; gen_typing.
       etransitivity. 2: gen_typing.
@@ -135,7 +146,7 @@ Proof.
     now eapply reflBoolRedTmEq.
   - intros ? NA t ? Ru red; inversion Ru; subst.
     assert [Γ |- A ≅ tEmpty]< wl > by (destruct NA; gen_typing).
-    assert [Γ |- t :⇒*: nf : tEmpty]< wl >. 1:{
+    assert [Γ |- t :⤳*: nf : tEmpty]< wl >. 1:{
       constructor. 
       1: eapply ty_conv; gen_typing.
       etransitivity. 2: gen_typing.
@@ -144,29 +155,43 @@ Proof.
     split; econstructor; tea.
     now eapply reflEmptyRedTmEq.
     Unshelve. 2: tea.
+  - intros ? PA ihdom ihcod ?? ru' ?; pose (ru := ru'); destruct ru' as [p].
+    assert [Γ |- A ≅ PA.(outTy)]< wl >. 1:{
+      destruct PA as [?? []]. cbn in *.
+      eapply convty_exp; tea.
+      now apply redtywf_refl.
+    }
+    assert [Γ |-[ ta ] t ⤳* u : PA.(outTy)]< wl > by now eapply redtm_conv. 
+    assert [Γ |-[ ta ] t : PA.(outTy)]< wl > by (eapply ty_conv; gen_typing).
+    unshelve refine (let rt : [LRSig' PA | Γ ||- t : A]< wl > := _ in _).
+    1: unshelve eexists p _ _; tea; constructor; destruct red; tea; etransitivity; tea.
+    split; tea; exists rt ru sndTree; tea; intros; cbn; now apply reflLRTmEq.
+  - intros ? IA ih _ t u [nf ?? prop] redt.
+    assert [Γ |- A ≅ IA.(IdRedTy.outTy)]< wl > by (destruct IA; unfold IdRedTy.outTy; cbn; gen_typing).
+    assert [Γ |-[ ta ] t ⤳* u : IA.(IdRedTy.outTy)]< wl > by now eapply redtm_conv. 
+    assert [Γ |-[ ta ] t : IA.(IdRedTy.outTy)]< wl > by (eapply ty_conv; gen_typing).
+    assert [Γ |-[ ta ] t :⤳*: nf : IA.(IdRedTy.outTy)]< wl >.
+    1: constructor; [apply red|etransitivity; tea; apply red].
+    split; eexists; tea.
+    now eapply reflIdPropEq.
 Qed.
 
 Lemma WredSubstTerm {wl Γ A t u l}
   (RA : W[Γ ||-<l> A]< wl >) :
   W[Γ ||-<l> u : A | RA]< wl > ->
-  [Γ |- t ⇒* u : A ]< wl > ->
+  [Γ |- t ⤳* u : A ]< wl > ->
   W[Γ ||-<l> t : A | RA]< wl > × W[Γ ||-<l> t ≅ u : A | RA]< wl >.
 Proof.
   intros [] ?.
-  split ; exists WNTm.
-  - intros.
-    eapply redSubstTerm.
-    + now eapply WRedTm.
-    + now eapply redtm_Ltrans.
-  - intros.
-    eapply redSubstTerm.
-    + now eapply WRedTm.
-    + now eapply redtm_Ltrans.
+  split ; exists WTTm ; intros.
+  all: pose proof (Hyp := over_tree_le Hover).
+  all: eapply redSubstTerm ; [now eapply WRedTm | ].
+  all: now eapply redtm_Ltrans.
 Qed.
 
 Lemma redwfSubstTerm {wl Γ A t u l} (RA : [Γ ||-<l> A]< wl >) :
   [Γ ||-<l> u : A | RA]< wl > ->
-  [Γ |- t :⇒*: u : A ]< wl > ->
+  [Γ |- t :⤳*: u : A ]< wl > ->
   [Γ ||-<l> t : A | RA]< wl > × [Γ ||-<l> t ≅ u : A | RA]< wl >.
 Proof.
   intros ? []; now eapply redSubstTerm.
@@ -175,54 +200,70 @@ Qed.
 
 Lemma redFwd {wl Γ l A B} :
   [Γ ||-<l> A]< wl > ->
-  [Γ |- A :⇒*: B]< wl > ->
+  [Γ |- A :⤳*: B]< wl > ->
   whnf B ->
   [Γ ||-<l> B]< wl >.
 Proof.
   intros RA; revert B; pattern l, wl, Γ, A, RA; apply LR_rect_TyUr; clear l wl Γ A RA.
   - intros ???? [??? red] ? red' ?. 
-    eapply LRU_.  unshelve erewrite (redtywf_det _ _ _ _ _ _ _ red' red); tea.
+    eapply LRU_.  unshelve erewrite (redtywf_det _ _ red' red); tea.
     1: constructor. econstructor; tea. eapply redtywf_refl; gen_typing.
   - intros ???? [? red] ? red' ?.
     eapply LRne_.
-    unshelve erewrite (redtywf_det _ _ _ _ _ _ _ red' red); tea.
-    1: constructor; now eapply ty_ne_whne.
+    unshelve erewrite (redtywf_det _ _ red' red); tea.
+    1: constructor; now eapply convneu_whne.
     econstructor; tea.
     eapply redtywf_refl; gen_typing.
   - intros ???? [?? red] ?? ? red' ?.
     eapply LRPi'. 
-    unshelve erewrite (redtywf_det _ _ _ _ _ _ _ red' red); tea.
+    unshelve erewrite (redtywf_det _ _ red' red); tea.
     1: constructor.
-    econstructor; tea.
-    eapply redtywf_refl; gen_typing.
+    econstructor.
+    + eapply redtywf_refl; gen_typing.
+    + eassumption.
+    + eassumption.
+    + eassumption.
   - intros ???? [red] ? red' ?.
     eapply LRNat_.
-    unshelve erewrite (redtywf_det _ _ _ _ _ _ _ red' red); tea.
+    unshelve erewrite (redtywf_det _ _ red' red); tea.
     1: constructor.
     econstructor; tea.
     eapply redtywf_refl; gen_typing.
   - intros ???? [red] ? red' ?.
     eapply LRBool_.
-    unshelve erewrite (redtywf_det _ _ _ _ _ _ _ red' red); tea.
+    unshelve erewrite (redtywf_det _ _ red' red); tea.
     1: constructor.
     econstructor; tea.
     eapply redtywf_refl; gen_typing.
   - intros ???? [red] ? red' ?.
     eapply LREmpty_.
-    unshelve erewrite (redtywf_det _ _ _ _ _ _ _ red' red); tea.
+    unshelve erewrite (redtywf_det _ _ red' red); tea.
     1: constructor.
     econstructor; tea.
     eapply redtywf_refl; gen_typing.
+  - intros ???? [?? red] ?? ? red' ?.
+    eapply LRSig'. 
+    unshelve erewrite (redtywf_det _ _ red' red); tea.
+    1: constructor.
+    econstructor.
+    + eapply redtywf_refl; gen_typing.
+    + eassumption.
+    + eassumption.
+    + eassumption.
+  - intros ???? [???? red] _ _ ? red' ?.
+    eapply LRId'; unshelve erewrite (redtywf_det _ _ red' red); tea; [constructor|].
+    econstructor; tea. eapply redtywf_refl; gen_typing.
 Qed.
 
 Lemma WredFwd {wl Γ l A B} :
   W[Γ ||-<l> A]< wl > ->
-  [Γ |- A :⇒*: B]< wl > ->
+  [Γ |- A :⤳*: B]< wl > ->
   whnf B ->
   W[Γ ||-<l> B]< wl >.
 Proof.
   intros [] red whB.
-  exists WN ; intros.
+  exists WT ; intros.
+  pose proof (Hyp := over_tree_le Ho).
   unshelve eapply redFwd.
   - exact A.
   - now eapply WRed.
@@ -233,15 +274,26 @@ Proof.
 Qed.
 
 
+Lemma redFwdConv {wl Γ l A B} (RA : [Γ ||-<l> A]< wl >) : [Γ |- A :⤳*: B]< wl > -> whnf B -> [Γ ||-<l> B]< wl > × [Γ ||-<l> A ≅ B | RA]< wl >.
+Proof.
+  intros red wh. pose (RB := redFwd RA red wh).
+  destruct (redwfSubst RB red).
+  split; tea; irrelevance.
+Qed.
+
+Lemma IdProp_whnf {wl Γ l A} (IA : [Γ ||-Id<l> A]< wl >) t : IdProp IA t -> whnf t.
+Proof. intros []; constructor; destruct r; now eapply convneu_whne. Qed.
+
+
 Lemma redTmFwd {wl Γ l A t u} {RA : [Γ ||-<l> A]< wl >} : 
   [Γ ||-<l> t : A | RA]< wl > ->
-  [Γ |- t :⇒*: u : A]< wl > ->
+  [Γ |- t :⤳*: u : A]< wl > ->
   whnf u ->
   [Γ ||-<l> u : A | RA]< wl >.
 Proof.
   revert t u; pattern l,wl, Γ,A,RA; apply LR_rect_TyUr; clear l wl Γ A RA.
   - intros ??????? [? red] red' ?.
-    unshelve erewrite (redtmwf_det _ _ _ _ _ _ _ _ _ red' red); tea.
+    unshelve erewrite (redtmwf_det _ _ red' red); tea.
     1: now eapply isType_whnf.
     econstructor; tea.
     1: eapply redtmwf_refl; gen_typing.
@@ -249,41 +301,52 @@ Proof.
     2,3: gen_typing.
     now eapply RedTyRecFwd.
   - intros ???? ??? [? red] red' ?.
-    unshelve erewrite (redtmwf_det _ _ _ _ _ _ _ _ _ red' red); tea.
-    1: constructor; now eapply tm_ne_whne.
+    unshelve erewrite (redtmwf_det _ _ red' red); tea.
+    1: constructor; now eapply convneu_whne.
     econstructor; tea.
     eapply redtmwf_refl; gen_typing.
   - intros ????????? [? red] red' ?.
-    unshelve erewrite (redtmwf_det _ _ _ _ _ _ _ _ _ red' red); tea.
-    1: now eapply isFun_whnf.
+    unshelve erewrite (redtmwf_det _ _ red' red); tea.
+    1: eapply isFun_whnf; destruct isfun; constructor; tea; now eapply convneu_whne.
     econstructor; tea.
     eapply redtmwf_refl; gen_typing.
   - intros ??????? Rt red' ?; inversion Rt; subst.
-    unshelve erewrite (redtmwf_det _ _ _ _ _ _ _ _ _ red' red); tea.
+    unshelve erewrite (redtmwf_det _ _ red' red); tea.
     1: now eapply NatProp_whnf.
     econstructor; tea.
     eapply redtmwf_refl; gen_typing.
   - intros ??????? Rt red' ?; inversion Rt; subst.
-    unshelve erewrite (redtmwf_det _ _ _ _ _ _ _ _ _ red' red); tea.
+    unshelve erewrite (redtmwf_det _ _ red' red); tea.
     1: now eapply BoolProp_whnf.
     econstructor; tea.
     eapply redtmwf_refl; gen_typing.
   - intros ??????? Rt red' ?; inversion Rt; subst.
-    unshelve erewrite (redtmwf_det _ _ _ _ _ _ _ _ _ red' red); tea.
+    unshelve erewrite (redtmwf_det _ _ red' red); tea.
     1: now eapply EmptyProp_whnf.
     econstructor; tea.
     eapply redtmwf_refl; gen_typing.
     Unshelve. 2: tea.
+  - intros ????????? [? red] red' ?.
+    unshelve erewrite (redtmwf_det _ _ red' red); tea.
+    1: eapply isPair_whnf; destruct ispair; constructor; tea; now eapply convneu_whne.
+    econstructor; tea.
+    eapply redtmwf_refl; gen_typing.
+  - intros ????????? [? red] red' ?.
+    unshelve erewrite (redtmwf_det _ _ red' red); tea.
+    1: now eapply IdProp_whnf.
+    econstructor; tea.
+    eapply redtmwf_refl; gen_typing.
 Qed.
 
 Lemma WredTmFwd {wl Γ l A t u} {RA : W[Γ ||-<l> A]< wl >} : 
   W[Γ ||-<l> t : A | RA]< wl > ->
-  [Γ |- t :⇒*: u : A]< wl > ->
+  [Γ |- t :⤳*: u : A]< wl > ->
   whnf u ->
   W[Γ ||-<l> u : A | RA]< wl >.
 Proof.
   intros [] [wfA red] whu.
-  exists WNTm ; intros.
+  exists WTTm ; intros.
+  pose proof (Hyp := over_tree_le Hover).
   eapply redTmFwd ; try assumption.
   - now eapply WRedTm.
   - econstructor.
