theories/LogicalRelation/Split.v
@@ -1,0 +1,94 @@
+From LogRel.AutoSubst Require Import core unscoped Ast Extra.
+From LogRel Require Import Utils BasicAst Notations LContexts Context NormalForms Weakening GenericTyping Monad LogicalRelation.
+From LogRel.LogicalRelation Require Import Induction Irrelevance.
+
+Section Split.
+  Context `{GenericTypingProperties}.
+
+  Lemma Split@{i j k l} {wl : wfLCon} {lA Γ A} {n : nat} {ne : not_in_LCon wl n} :
+    WLogRel@{i j k l} lA (wl ,,l (ne, true)) Γ A ->
+    WLogRel@{i j k l} lA (wl ,,l (ne, false)) Γ A ->
+    WLogRel@{i j k l} lA wl Γ A.
+  Proof.
+    intros [WTt WRedt] [WTf WRedf].
+    exists (ϝnode _ WTt WTf).
+    intros wl' Hover.
+    cbn in *.
+    destruct (decidInLCon wl' n) ; [ | | now inversion Hover].
+    - now eapply WRedt.
+    - now eapply WRedf.
+  Defined.
+
+  Lemma EqSplit@{i j k l} {wl : wfLCon} {lA Γ A B} {n : nat} {ne : not_in_LCon wl n}
+    HAt HAf :
+    WLogRelEq@{i j k l} lA (wl ,,l (ne, true)) Γ A B HAt ->
+    WLogRelEq@{i j k l} lA (wl ,,l (ne, false)) Γ A B HAf ->
+    WLogRelEq@{i j k l} lA wl Γ A B (Split HAt HAf).
+  Proof.
+    intros [WTt WRedt] [WTf WRedf].
+    exists (ϝnode _ WTt WTf).
+    intros wl' Hover Hover' ; cbn in *.
+    destruct (decidInLCon wl' n) ; [ | | now inversion Hover].
+    - now eapply WRedt.
+    - now eapply WRedf.
+  Qed.
+
+  Corollary EqSplit'@{i j k l} {wl : wfLCon} {lA Γ A B} {n : nat} {ne : not_in_LCon wl n}
+    HAt HAf HA :
+    WLogRelEq@{i j k l} lA (wl ,,l (ne, true)) Γ A B HAt ->
+    WLogRelEq@{i j k l} lA (wl ,,l (ne, false)) Γ A B HAf ->
+    WLogRelEq@{i j k l} lA wl Γ A B HA.
+  Proof.
+    intros HBt HBf ; eapply WLRTyEqIrrelevant' ; [reflexivity | ].
+    eapply EqSplit ; eassumption.
+  Qed. 
+
+  Lemma TmSplit@{i j k l} {wl : wfLCon} {lA Γ t A} {n : nat} {ne : not_in_LCon wl n}
+    HAt HAf :
+    WLogRelTm@{i j k l} lA (wl ,,l (ne, true)) Γ t A HAt ->
+    WLogRelTm@{i j k l} lA (wl ,,l (ne, false)) Γ t A HAf ->
+    WLogRelTm@{i j k l} lA wl Γ t A (Split HAt HAf).
+  Proof.
+    intros [WTt WRedt] [WTf WRedf].
+    exists (ϝnode _ WTt WTf).
+    intros wl' Hover Hover' ; cbn in *.
+    destruct (decidInLCon wl' n) ; [ | | now inversion Hover].
+    - now eapply WRedt.
+    - now eapply WRedf.
+  Qed.
+
+  Corollary TmSplit'@{i j k l} {wl : wfLCon} {lA Γ t A} {n : nat} {ne : not_in_LCon wl n}
+    HAt HAf HA :
+    WLogRelTm@{i j k l} lA (wl ,,l (ne, true)) Γ t A HAt ->
+    WLogRelTm@{i j k l} lA (wl ,,l (ne, false)) Γ t A HAf ->
+    WLogRelTm@{i j k l} lA wl Γ t A HA.
+  Proof.
+    intros Htt Htf ; eapply WLRTmRedIrrelevant' ; [reflexivity | ].
+    eapply TmSplit ; eassumption.
+  Qed. 
+
+  Lemma TmEqSplit@{i j k l} {wl : wfLCon} {lA Γ t u A} {n : nat} {ne : not_in_LCon wl n}
+    HAt HAf :
+    WLogRelTmEq@{i j k l} lA (wl ,,l (ne, true)) Γ t u A HAt ->
+    WLogRelTmEq@{i j k l} lA (wl ,,l (ne, false)) Γ t u A HAf ->
+    WLogRelTmEq@{i j k l} lA wl Γ t u A (Split HAt HAf).
+  Proof.
+    intros [WTt WRedt] [WTf WRedf].
+    exists (ϝnode _ WTt WTf).
+    intros wl' Hover Hover' ; cbn in *.
+    destruct (decidInLCon wl' n) ; [ | | now inversion Hover].
+    - now eapply WRedt.
+    - now eapply WRedf.
+  Qed.
+
+  Lemma TmEqSplit'@{i j k l} {wl : wfLCon} {lA Γ t u A} {n : nat} {ne : not_in_LCon wl n}
+    HAt HAf HA :
+    WLogRelTmEq@{i j k l} lA (wl ,,l (ne, true)) Γ t u A HAt ->
+    WLogRelTmEq@{i j k l} lA (wl ,,l (ne, false)) Γ t u A HAf ->
+    WLogRelTmEq@{i j k l} lA wl Γ t u A HA.
+  Proof.
+    intros Htt Htf ; eapply WLRTmEqIrrelevant' ; [reflexivity | ].
+    eapply TmEqSplit ; eassumption.
+  Qed. 
+  
+End Split.
